Finish proof for new rs controller impl; need to revisit go_size_safe

src/proof/k8s_io/apimachinery/pkg/labels_init.v
@@ -1,5 +1,10 @@
 Require Export New.generatedproof.k8s_io.apimachinery.pkg.labels.
 From New.proof Require Import proof_prelude.
+From New.proof Require Export sort_init strconv_init.
+From New.proof.k8s_io.klog Require Export klog_init.
+From New.proof.k8s_io.apimachinery.pkg Require Export selection_init.
+From New.proof.k8s_io.apimachinery.pkg.util Require Export validation_init.
+From New.proof.k8s_io.apimachinery.pkg.util.validation Require Export field_init.
 
 
 Section proof.
@@ -7,7 +12,14 @@ Context `{hG: heapGS Σ} `{!ffi_semantics _ _}.
 Context {sem : go.Semantics} {package_sem : labels.Assumptions}.
 Collection W := sem + package_sem.
 
-#[global] Instance : IsPkgInit (iProp Σ) labels := define_is_pkg_init True%I.
+Definition is_initialized : iProp Σ :=
+  "#Heverything" ∷ (global_addr labels.sharedEverythingSelector) ↦□
+    interface.ok (interface.mk labels.internalSelector #slice.nil) ∗
+  "#Hnothing" ∷ (global_addr labels.sharedNothingSelector) ↦□
+    interface.ok (interface.mk labels.nothingSelector #(labels.nothingSelector.mk)).
+
+#[global] Instance : IsPkgInit (iProp Σ) labels :=
+  define_is_pkg_init is_initialized.
 #[global] Instance : GetIsPkgInitWf (iProp Σ) labels := build_get_is_pkg_init_wf.
 
 End proof.
