src/proof/controllers/replicaset/get_indirectly_related_pods.v
@@ -1,6 +1,7 @@
 From New.proof Require Import prelude empty_ffi.
 From New.proof.controllers.replicaset Require Export get_replica_sets_with_same_controller.
-From New.proof.kubernetes_model Require Export inv.
+From New.proof.k8s_io.apimachinery.pkg.apis.meta Require Export
+  v1_label_selector_as_selector.
 
 Section proof.
 Context `{hG: !heapGS Σ} `{!ffi_semantics _ _}.
@@ -45,6 +46,324 @@ Lemma wp_getIndirectlyRelatedPods γ l rs_l rs dq :
       ([∗ list] ptr;pod ∈ ptrs;pods, PodV.deepown_l ptr pod dq') ∗
       ReplicaSetV.deepown_l rs_l rs dq
   }}}.
-Proof. Admitted.
+Proof.
+  wp_start as "H". iNamed "H".
+  iDestruct "Hisk" as "#Hisk".
+  iDestruct "Hglobal_l" as "#Hglobal_l".
+  iAssert (is_pkg_init v1) as "#Hmeta_init".
+  { iPkgInit. }
+  iAssert (is_pkg_init apimodel) as "#Hapimodel_init".
+  { iPkgInit. }
+  wp_auto.
+  wp_apply (wp_getReplicaSetsWithSameController γ l rs_l rs dq with
+    "[$Hrs $Hisk $Hglobal_l]").
+  iIntros (related_sets_sl related_set_ptrs related_sets related_dq)
+    "(Hrelated_sets_sl & Hrelated_sets & %Hrelated_sets_valid & Hrs)".
+  wp_auto.
+  wp_apply wp_slice_literal. iSplitR; first done.
+  iIntros (result_backing_l) "[Hresult_sl Hresult_cap]". wp_auto.
+  wp_apply wp_map_make1 as (seen_l) "Hseen".
+  iDestruct (own_slice_len with "Hrelated_sets_sl") as
+    %(Hrelated_sets_len1 & Hrelated_sets_len2).
+  iDestruct (big_sepL2_length with "Hrelated_sets") as
+    %Hrelated_sets_len.
+  set I := (∃ (i : w64) (related_rs_l : loc) (result_sl' : slice.t)
+      (result_ptrs : list loc) (result_pods : list PodV.t)
+      (seen : gmap types.UID.t loc),
+    "Hi_ptr" ∷ i_ptr ↦ i ∗
+    "Hrelated_rs_ptr" ∷ relatedRS_ptr ↦ related_rs_l ∗
+    "Hresult_ptr" ∷ relatedPods_ptr ↦ result_sl' ∗
+    "Hseen_ptr" ∷ seen_ptr ↦ seen_l ∗
+    "Hresult_sl" ∷ result_sl' ↦* result_ptrs ∗
+    "Hresult_cap" ∷ own_slice_cap loc result_sl' (DfracOwn 1) ∗
+    "Hresult_pods" ∷
+      ([∗ list] ptr;pod ∈ result_ptrs;result_pods,
+        PodV.deepown_l ptr pod 1) ∗
+    "Hseen" ∷ seen_l ↦$ seen ∗
+    "Hrelated_sets" ∷
+      ([∗ list] ptr;related_rs ∈ related_set_ptrs;related_sets,
+        ReplicaSetV.deepown_l ptr related_rs related_dq) ∗
+    "%Hi" ∷
+      ⌜ 0 ≤ sint.Z i ≤ sint.Z (slice.len related_sets_sl) ⌝)%I.
+  iAssert I with
+    "[i relatedRS relatedPods seen Hresult_sl Hresult_cap Hseen
+      Hrelated_sets]" as "Houter".
+  { iExists (W64 0), null,
+      (slice.mk result_backing_l (W64 0) (W64 0)), [], [], ∅.
+    iFrame. rewrite big_sepL2_nil. iFrame. iPureIntro. word. }
+  wp_for "Houter". wp_if_destruct.
+  - list_elem related_set_ptrs (sint.Z i) as this_rs_l.
+    destruct (decide
+      (0 ≤ sint.Z i < sint.Z (slice.len related_sets_sl))) as
+      [_|Hbounds]; last word.
+    wp_apply (wp_load_slice_index with "[$Hrelated_sets_sl]");
+      [word|iPureIntro; exact Hthis_rs_l_lookup|].
+    iIntros "Hrelated_sets_sl". wp_auto.
+    assert (∃ this_rs, related_sets !! sint.nat i = Some this_rs) as
+      [this_rs Hthis_rs_lookup].
+    { apply lookup_lt_is_Some_2.
+      rewrite -Hrelated_sets_len Hrelated_sets_len1. word. }
+    assert (ReplicaSetV.valid this_rs) as Hthis_rs_valid.
+    { rewrite Forall_forall in Hrelated_sets_valid.
+      apply Hrelated_sets_valid.
+      rewrite <-list_elem_of_In.
+      apply list_elem_of_lookup_2 with (i:=sint.nat i).
+      exact Hthis_rs_lookup. }
+    iDestruct (big_sepL2_lookup_acc with "Hrelated_sets") as
+      "[Hthis_rs Hrestore_related_sets]";
+      [exact Hthis_rs_l_lookup|exact Hthis_rs_lookup|].
+    destruct Hthis_rs_valid as
+      (_ & _ & _ & [(_ & _ &
+        (api_selector & Hapi_selector_eq & Hapi_selector_valid & _) & _) _]
+        & _).
+    iPoseProof (ReplicaSetV.deepown_l_split with "Hthis_rs") as
+      "(%Hthis_rs_nonnull & Hthis_rs_type & Hthis_rs_meta_l &
+        Hthis_rs_spec & Hthis_rs_status)".
+    iDestruct "Hthis_rs_spec" as (this_rs_spec_c)
+      "[Hthis_rs_spec_l Hthis_rs_spec]".
+    iDestruct (struct_fields_split (V:=v1.ReplicaSetSpec.t) with
+      "Hthis_rs_spec_l") as
+      "[Hthis_rs_spec_fields %Hthis_rs_spec_nonnull]".
+    iNamedPrefix "Hthis_rs_spec_fields" "Hthis_rs_spec_field_".
+    iNamedPrefix "Hthis_rs_spec" "Hthis_rs_spec_deepown_".
+    iEval (rewrite Hapi_selector_eq) in
+      "Hthis_rs_spec_deepown_Hdeepown_selector_some".
+    wp_auto.
+    wp_apply (wp_LabelSelectorAsSelector with
+      "[$Hmeta_init
+        $Hthis_rs_spec_deepown_Hdeepown_selector_some]"); first done.
+    iIntros (selector)
+      "(Hthis_rs_spec_deepown_Hdeepown_selector_some & #Hselector)".
+    iCombineNamed "Hthis_rs_spec_field_*" as "Hthis_rs_spec_fields".
+    iAssert (typed_pointsto_def (ReplicaSetV.spec_ptr this_rs_l)
+        this_rs_spec_c related_dq) with "[Hthis_rs_spec_fields]" as
+      "Hthis_rs_spec_l".
+    { iNamed "Hthis_rs_spec_fields". simpl. rewrite /named. iFrame. }
+    iDestruct (struct_fields_combine (V:=v1.ReplicaSetSpec.t)
+      (ReplicaSetV.spec_ptr this_rs_l) this_rs_spec_c related_dq
+      Hthis_rs_spec_nonnull with "Hthis_rs_spec_l") as
+      "Hthis_rs_spec_l".
+    iAssert (ReplicaSetSpecV.deepown this_rs_spec_c
+        this_rs.(ReplicaSetV.Spec') related_dq)
+      with "[Hthis_rs_spec_deepown_Hdeepown_replicas_some
+        Hthis_rs_spec_deepown_Hdeepown_selector_some
+        Hthis_rs_spec_deepown_Hdeepown_template]" as "Hthis_rs_spec".
+    { rewrite /ReplicaSetSpecV.deepown /named Hapi_selector_eq.
+      iFrame. iFrame "%". iPureIntro.
+      rewrite Hapi_selector_eq in
+        Hthis_rs_spec_deepown_Hdeepown_selector_none.
+      exact Hthis_rs_spec_deepown_Hdeepown_selector_none. }
+    iAssert (ReplicaSetSpecV.deepown_l (ReplicaSetV.spec_ptr this_rs_l)
+        this_rs.(ReplicaSetV.Spec') related_dq)
+      with "[Hthis_rs_spec_l Hthis_rs_spec]" as "Hthis_rs_spec".
+    { iExists this_rs_spec_c. iFrame. }
+    iDestruct "Hthis_rs_meta_l" as (this_rs_meta_c)
+      "[Hthis_rs_meta_l Hthis_rs_meta]".
+    iDestruct (struct_fields_split (V:=v1.ObjectMeta.t) with
+      "Hthis_rs_meta_l") as
+      "[Hthis_rs_meta_fields %Hthis_rs_meta_nonnull]".
+    iNamedPrefix "Hthis_rs_meta_fields" "Hthis_rs_meta_field_".
+    iNamedPrefix "Hthis_rs_meta" "Hthis_rs_meta_deepown_".
+    wp_auto.
+    rewrite Hthis_rs_meta_deepown_Hdeepown_namespace.
+    wp_apply (wp_State__PodList_weak γ l
+      this_rs.(ReplicaSetV.ObjectMeta').(ObjectMetaV.Namespace') selector
+      (LabelSelectorV.matches api_selector)
+      (H:=λ labels : option (gmap go_string go_string),
+        LabelSelectorV.matches_dec api_selector labels)
+      with "[$Hapimodel_init $Hselector $Hisk]").
+    iIntros (pods_sl pod_ptrs pods)
+      "(Hpods_sl & Hpods & %Hpods_valid)".
+    iCombineNamed "Hthis_rs_meta_field_*" as "Hthis_rs_meta_fields".
+    iAssert (typed_pointsto_def (ReplicaSetV.objectmeta_ptr this_rs_l)
+        this_rs_meta_c related_dq) with "[Hthis_rs_meta_fields]" as
+      "Hthis_rs_meta_l".
+    { iNamed "Hthis_rs_meta_fields". simpl. rewrite /named.
+      rewrite Hthis_rs_meta_deepown_Hdeepown_namespace. iFrame. }
+    iDestruct (struct_fields_combine (V:=v1.ObjectMeta.t)
+      (ReplicaSetV.objectmeta_ptr this_rs_l) this_rs_meta_c related_dq
+      Hthis_rs_meta_nonnull with "Hthis_rs_meta_l") as
+      "Hthis_rs_meta_l".
+    iCombineNamed "Hthis_rs_meta_deepown_*" as
+      "Hthis_rs_meta_deepown".
+    iAssert (ObjectMetaV.deepown this_rs_meta_c
+        this_rs.(ReplicaSetV.ObjectMeta') related_dq)
+      with "[Hthis_rs_meta_deepown]" as "Hthis_rs_meta".
+    { iNamed "Hthis_rs_meta_deepown".
+      rewrite /ObjectMetaV.deepown /named. iFrame. iFrame "%". }
+    iAssert (ObjectMetaV.deepown_l
+        (ReplicaSetV.objectmeta_ptr this_rs_l)
+        this_rs.(ReplicaSetV.ObjectMeta') related_dq)
+      with "[Hthis_rs_meta_l Hthis_rs_meta]" as "Hthis_rs_meta_l".
+    { iExists this_rs_meta_c. iFrame. }
+    iPoseProof (ReplicaSetV.deepown_l_restore _ _ _ Hthis_rs_nonnull with
+      "[$Hthis_rs_type $Hthis_rs_meta_l $Hthis_rs_spec
+        $Hthis_rs_status]") as "Hthis_rs".
+    iPoseProof ("Hrestore_related_sets" with "Hthis_rs") as
+      "Hrelated_sets".
+    wp_auto.
+    iDestruct (own_slice_len with "Hpods_sl") as
+      %(Hpods_len1 & Hpods_len2).
+    iDestruct (big_sepL2_length with "Hpods") as %Hpods_len.
+    wp_alloc j_ptr as "j".
+    set J := (∃ (j : w64) (pod_l : loc) (result_sl'' : slice.t)
+        (result_ptrs' : list loc) (result_pods' : list PodV.t)
+        (seen' : gmap types.UID.t loc),
+      "Hj_ptr" ∷ j_ptr ↦ j ∗
+      "Hpod_ptr" ∷ pod_ptr ↦ pod_l ∗
+      "Hrelated_rs_ptr" ∷ relatedRS_ptr ↦ this_rs_l ∗
+      "Hresult_ptr" ∷ relatedPods_ptr ↦ result_sl'' ∗
+      "Hseen_ptr" ∷ seen_ptr ↦ seen_l ∗
+      "Hresult_sl" ∷ result_sl'' ↦* result_ptrs' ∗
+      "Hresult_cap" ∷ own_slice_cap loc result_sl'' (DfracOwn 1) ∗
+      "Hresult_pods" ∷
+        ([∗ list] ptr;pod ∈ result_ptrs';result_pods',
+          PodV.deepown_l ptr pod 1) ∗
+      "Hseen" ∷ seen_l ↦$ seen' ∗
+      "Hpods_post" ∷
+        ([∗ list] ptr;pod ∈ drop (sint.nat j) pod_ptrs;
+          drop (sint.nat j) pods, PodV.deepown_l ptr pod 1) ∗
+      "Hrelated_sets" ∷
+        ([∗ list] ptr;related_rs ∈ related_set_ptrs;related_sets,
+          ReplicaSetV.deepown_l ptr related_rs related_dq) ∗
+      "%Hj" ∷ ⌜ 0 ≤ sint.Z j ≤ sint.Z (slice.len pods_sl) ⌝)%I.
+    iAssert J with
+      "[j pod Hrelated_rs_ptr Hresult_ptr Hseen_ptr Hresult_sl
+        Hresult_cap Hresult_pods Hseen Hpods Hrelated_sets]" as "Hinner".
+    { iExists (W64 0), null, result_sl', result_ptrs, result_pods, seen.
+      iFrame. iPureIntro. word. }
+    wp_auto.
+    wp_for "Hinner". wp_if_destruct.
+    + list_elem pod_ptrs (sint.Z j) as this_pod_l.
+      destruct (decide
+        (0 ≤ sint.Z j < sint.Z (slice.len pods_sl))) as
+        [_|Hpod_bounds]; last word.
+      wp_apply (wp_load_slice_index with "[$Hpods_sl]");
+        [word|iPureIntro; exact Hthis_pod_l_lookup|].
+      iIntros "Hpods_sl". wp_auto.
+      assert (∃ this_pod, pods !! sint.nat j = Some this_pod) as
+        [this_pod Hthis_pod_lookup].
+      { apply lookup_lt_is_Some_2.
+        rewrite -Hpods_len Hpods_len1. word. }
+      iPoseProof (big_sepL2_head_tail _ _ _ this_pod_l this_pod with
+        "Hpods_post") as "[Hthis_pod Hother_pods]".
+      { split. all: rewrite lookup_drop Nat.add_0_r; done. }
+      iPoseProof (PodV.deepown_l_split with "Hthis_pod") as
+        "(%Hthis_pod_nonnull & Hthis_pod_type & Hthis_pod_meta_l &
+          Hthis_pod_spec & Hthis_pod_status)".
+      iDestruct "Hthis_pod_meta_l" as (this_pod_meta_c)
+        "[Hthis_pod_meta_l Hthis_pod_meta]".
+      iDestruct (struct_fields_split (V:=v1.ObjectMeta.t) with
+        "Hthis_pod_meta_l") as
+        "[Hthis_pod_meta_fields %Hthis_pod_meta_nonnull]".
+      iNamedPrefix "Hthis_pod_meta_fields" "Hthis_pod_meta_field_".
+      iNamedPrefix "Hthis_pod_meta" "Hthis_pod_meta_deepown_".
+      wp_auto.
+      rewrite Hthis_pod_meta_deepown_Hdeepown_uid.
+      wp_apply (wp_map_lookup2 types.UID
+        (go.PointerType api_apps_v1.ReplicaSet) with "[$Hseen]").
+      iIntros "Hseen".
+      destruct (seen' !!
+        this_pod.(PodV.ObjectMeta').(ObjectMetaV.UID')) as
+        [seen_rs_l|] eqn:Hseen_lookup; wp_auto.
+      * iCombineNamed "Hthis_pod_meta_field_*" as
+          "Hthis_pod_meta_fields".
+        iAssert (typed_pointsto_def (PodV.objectmeta_ptr this_pod_l)
+            this_pod_meta_c 1) with "[Hthis_pod_meta_fields]" as
+          "Hthis_pod_meta_l".
+        { iNamed "Hthis_pod_meta_fields". simpl. rewrite /named.
+          rewrite Hthis_pod_meta_deepown_Hdeepown_uid. iFrame. }
+        iDestruct (struct_fields_combine (V:=v1.ObjectMeta.t)
+          (PodV.objectmeta_ptr this_pod_l) this_pod_meta_c 1
+          Hthis_pod_meta_nonnull with "Hthis_pod_meta_l") as
+          "Hthis_pod_meta_l".
+        iCombineNamed "Hthis_pod_meta_deepown_*" as
+          "Hthis_pod_meta_deepown".
+        iAssert (ObjectMetaV.deepown this_pod_meta_c
+            this_pod.(PodV.ObjectMeta') 1)
+          with "[Hthis_pod_meta_deepown]" as "Hthis_pod_meta".
+        { iNamed "Hthis_pod_meta_deepown".
+          rewrite /ObjectMetaV.deepown /named. iFrame. iFrame "%". }
+        iAssert (ObjectMetaV.deepown_l (PodV.objectmeta_ptr this_pod_l)
+            this_pod.(PodV.ObjectMeta') 1)
+          with "[Hthis_pod_meta_l Hthis_pod_meta]" as
+          "Hthis_pod_meta_l".
+        { iExists this_pod_meta_c. iFrame. }
+        iPoseProof (PodV.deepown_l_restore _ _ _ Hthis_pod_nonnull with
+          "[$Hthis_pod_type $Hthis_pod_meta_l $Hthis_pod_spec
+            $Hthis_pod_status]") as "Hthis_pod".
+        iApply wp_for_post_continue. wp_auto.
+        iFrame "Hpods_sl Hrelated_sets_sl HΦ Hrs".
+        iFrame "Hi_ptr".
+        iExists (word.add j (W64 1)), this_pod_l, result_sl'',
+          result_ptrs', result_pods', seen'.
+        assert (sint.nat (word.add j (W64 1)) = S (sint.nat j)) as
+          -> by word.
+        rewrite !drop_drop Nat.add_1_r. iFrame. iPureIntro. word.
+      * iCombineNamed "Hthis_pod_meta_field_*" as
+          "Hthis_pod_meta_fields".
+        iAssert (typed_pointsto_def (PodV.objectmeta_ptr this_pod_l)
+            this_pod_meta_c 1) with "[Hthis_pod_meta_fields]" as
+          "Hthis_pod_meta_l".
+        { iNamed "Hthis_pod_meta_fields". simpl. rewrite /named.
+          rewrite Hthis_pod_meta_deepown_Hdeepown_uid. iFrame. }
+        iDestruct (struct_fields_combine (V:=v1.ObjectMeta.t)
+          (PodV.objectmeta_ptr this_pod_l) this_pod_meta_c 1
+          Hthis_pod_meta_nonnull with "Hthis_pod_meta_l") as
+          "Hthis_pod_meta_l".
+        iCombineNamed "Hthis_pod_meta_deepown_*" as
+          "Hthis_pod_meta_deepown".
+        iAssert (ObjectMetaV.deepown this_pod_meta_c
+            this_pod.(PodV.ObjectMeta') 1)
+          with "[Hthis_pod_meta_deepown]" as "Hthis_pod_meta".
+        { iNamed "Hthis_pod_meta_deepown".
+          rewrite /ObjectMetaV.deepown /named. iFrame. iFrame "%". }
+        iAssert (ObjectMetaV.deepown_l (PodV.objectmeta_ptr this_pod_l)
+            this_pod.(PodV.ObjectMeta') 1)
+          with "[Hthis_pod_meta_l Hthis_pod_meta]" as
+          "Hthis_pod_meta_l".
+        { iExists this_pod_meta_c. iFrame. }
+        iPoseProof (PodV.deepown_l_restore _ _ _ Hthis_pod_nonnull with
+          "[$Hthis_pod_type $Hthis_pod_meta_l $Hthis_pod_spec
+            $Hthis_pod_status]") as "Hthis_pod".
+        wp_apply (wp_map_insert types.UID with "[$Hseen]") as "Hseen".
+        wp_apply wp_slice_literal. iSplitR; first done.
+        iIntros (one_sl) "[Hone_sl _]". wp_auto.
+        wp_apply (wp_slice_append with
+          "[$Hresult_sl $Hresult_cap $Hone_sl]").
+        iIntros (result_sl''')
+          "(Hresult_sl & Hresult_cap & Hone_sl)". wp_auto.
+        iAssert (([∗ list] ptr;pod ∈
+            result_ptrs' ++ [this_pod_l];result_pods' ++ [this_pod],
+            PodV.deepown_l ptr pod 1))%I
+          with "[Hresult_pods Hthis_pod]" as "Hresult_pods".
+        { iApply (big_sepL2_app with "[$Hresult_pods]").
+          simpl. iFrame. }
+        iApply wp_for_post_do. wp_auto.
+        iFrame "Hpods_sl Hrelated_sets_sl HΦ Hrs".
+        iFrame "Hi_ptr".
+        iExists (word.add j (W64 1)), this_pod_l, result_sl''',
+          (result_ptrs' ++ [this_pod_l]),
+          (result_pods' ++ [this_pod]),
+          (<[this_pod.(PodV.ObjectMeta').(ObjectMetaV.UID'):=this_rs_l]>
+            seen').
+        assert (sint.nat (word.add j (W64 1)) = S (sint.nat j)) as
+          -> by word.
+        rewrite !drop_drop Nat.add_1_r. iFrame. iPureIntro. word.
+    + clear J.
+      iApply wp_for_post_do. wp_auto.
+      iFrame "Hrelated_sets_sl HΦ Hrs".
+      iExists (word.add i (W64 1)), this_rs_l, result_sl'',
+        result_ptrs', result_pods', seen'.
+      iFrame.
+      iPureIntro. word.
+  - clear I. wp_auto.
+    iApply ("HΦ" $! result_sl' result_ptrs result_pods (DfracOwn 1)).
+    iFrame.
+
+Unshelve. all: try tc_solve.
+(* [wp_apply] leaves a proof-irrelevant label-map argument unconstrained. *)
+all: exact (None : option (gmap go_string go_string)).
+Qed.
 
 End proof.
