src/proof/k8s_io/apimachinery/pkg/apis/meta/v1_label_selector_as_selector.v
@@ -1,0 +1,1106 @@
+From New.proof Require Import prelude empty_ffi.
+From New.proof.map Require Import len for_range.
+From New.proof.k8s_io.apimachinery.pkg.apis.meta Require Export
+  v1 v1_label_selector_conversion.
+From New.proof.kubernetes_types Require Import labelselector.
+
+Section proof.
+Context `{hG: !heapGS Σ} `{!ffi_semantics _ _}.
+Context {sem : go.Semantics} {package_sem : v1.Assumptions}.
+Collection W := sem + package_sem.
+Local Set Default Proof Using "All".
+
+Lemma label_selector_matches_empty selector :
+  LabelSelectorV.empty selector →
+  ∀ labels_set,
+    LabelSelectorV.matches selector labels_set ↔ everything_matches labels_set.
+Proof.
+  intros ([Hlabels_none|Hlabels_empty] & Hexpressions) labels_set.
+  - rewrite /LabelSelectorV.matches /LabelSelectorV.match_labels
+      Hlabels_none Hexpressions /everything_matches /=. done.
+  - rewrite /LabelSelectorV.matches /LabelSelectorV.match_labels
+      Hlabels_empty Hexpressions /everything_matches /=.
+    destruct labels_set as [labels_set|]; simpl.
+    + done.
+    + split; [done|]. intros _. split; [done|constructor].
+Qed.
+
+Lemma wp_LabelSelectorAsSelector selector_l selector dq :
+  LabelSelectorV.executable selector →
+  {{{ is_pkg_init v1 ∗
+      LabelSelectorV.deepown_l selector_l selector dq
+  }}}
+    @! v1.LabelSelectorAsSelector #selector_l
+  {{{ converted, RET (#converted, #interface.nil);
+      LabelSelectorV.deepown_l selector_l selector dq ∗
+      is_selector converted (LabelSelectorV.matches selector)
+  }}}.
+Proof.
+  intros ((Hlabels_valid & Hexpressions_valid) & Hsize).
+  wp_start as "Hselector".
+  iAssert (is_pkg_init labels) as "#Hlabels_init".
+  { iPkgInit. }
+  iDestruct "Hselector" as (selector_c) "[Hselector_l Hselector]".
+  iDestruct (struct_fields_split (V:=v1.LabelSelector.t)
+    with "Hselector_l") as "[Hselector_fields %Hselector_nonnull]".
+  iNamedPrefix "Hselector_fields" "Hselector_field_".
+  iNamedPrefix "Hselector" "Hselector_".
+  wp_auto.
+  rewrite -> bool_decide_false by exact Hselector_nonnull.
+  wp_pures.
+  destruct selector.(LabelSelectorV.MatchLabels') as [labels_map|]
+    eqn:Hlabels_opt.
+  all: lazymatch goal with
+  | labels_map : gmap go_string go_string |- _ =>
+      iDestruct "Hselector_Hdeepown_matchlabels_some" as
+        (labels_map_c) "[Hlabels_map %Hlabels_map_c]";
+      subst labels_map_c
+  | _ =>
+      assert (v1.LabelSelector.MatchLabels' selector_c = map.nil)
+        as Hlabels_map_nil;
+      [apply (proj2 Hselector_Hdeepown_matchlabels_none); done|]
+  end.
+  all: destruct selector.(LabelSelectorV.MatchExpressions') as [expressions|]
+    eqn:Hexpressions_opt.
+  all: lazymatch goal with
+  | expressions : list LabelSelectorRequirementV.t |- _ =>
+      iDestruct "Hselector_Hdeepown_matchexpressions_some" as
+        (expressions_c) "Hexpressions";
+      iEval (rewrite /deepown_list) in "Hexpressions";
+      iDestruct "Hexpressions" as "[Hexpressions_sl Hexpressions]"
+  | _ =>
+      assert (v1.LabelSelector.MatchExpressions' selector_c = slice.nil)
+        as Hexpressions_nil;
+      [apply (proj2 Hselector_Hdeepown_matchexpressions_none); done|];
+      pose (expressions := ([] : list LabelSelectorRequirementV.t));
+      pose (expressions_c := ([] : list v1.LabelSelectorRequirement.t));
+      iAssert (v1.LabelSelector.MatchExpressions' selector_c ↦*
+        expressions_c)%I as "Hexpressions_sl";
+      [rewrite Hexpressions_nil /expressions_c; iApply own_slice_nil|];
+      iAssert (([∗ list] expression_c;expression ∈
+        expressions_c;expressions,
+        LabelSelectorRequirementV.deepown expression_c expression dq))%I
+        as "Hexpressions";
+      [rewrite /expressions_c /expressions big_sepL2_nil; done|]
+  end.
+  all: unfold LabelSelectorV.go_size_safe in Hsize.
+  all: rewrite Hlabels_opt /LabelSelectorV.match_expressions_list
+    Hexpressions_opt /= in Hsize.
+  all: try (rewrite Hlabels_opt /= in Hlabels_valid).
+  all: try (rewrite /LabelSelectorV.match_expressions_list
+    Hexpressions_opt /= in Hexpressions_valid).
+  all: iDestruct (own_slice_len with "Hexpressions_sl") as
+    %[Hexpressions_len Hexpressions_nonnegative].
+  all: iDestruct (big_sepL2_length with "Hexpressions") as
+    %Hexpressions_models_len.
+  all: assert (sint.nat
+      (slice.len (v1.LabelSelector.MatchExpressions' selector_c)) =
+      length expressions) as Hexpressions_word_len by lia.
+  all: wp_auto.
+  all: lazymatch goal with
+  | Hlabels_map_nil : _ = map.nil |- _ =>
+      rewrite Hlabels_map_nil;
+      wp_apply (wp_map_len_nil_resolved (K:=go_string) (V:=go_string)
+        go.string go.string)
+  | _ =>
+      wp_apply (wp_map_len_resolved (K:=go_string) (V:=go_string)
+        go.string go.string with "Hlabels_map");
+      iIntros "Hlabels_map"
+  end.
+  all: try done.
+  all: try (
+    wp_bind (![go.PointerType apis_meta_v1.LabelSelector] (#ps_ptr))%E;
+    wp_load;
+    wp_pure;
+    wp_bind (![go.SliceType apis_meta_v1.LabelSelectorRequirement]
+      (StructFieldRef apis_meta_v1.LabelSelector "MatchExpressions"
+        (#selector_l)))%E;
+    wp_pure;
+    wp_load;
+    wp_auto;
+    wp_if_destruct).
+  all: lazymatch goal with
+  | Hzero : word.add _ _ = W64 0 |- _ =>
+      assert (size (default ∅ selector.(LabelSelectorV.MatchLabels')) +
+        length expressions = 0)%nat as Hempty_sum by
+        (rewrite Hlabels_opt /=; word);
+      assert (length expressions = 0%nat) as Hexpressions_empty by lia;
+      apply nil_length_inv in Hexpressions_empty;
+      subst expressions
+  | _ => idtac
+  end.
+  all: try lazymatch goal with
+  | Hzero : word.add _ _ = W64 0,
+      labels_map : gmap go_string go_string |- _ =>
+      assert (size labels_map = 0%nat) as Hlabels_empty by
+        (rewrite Hlabels_opt /= in Hempty_sum; lia);
+      apply map_size_empty_inv in Hlabels_empty;
+      subst labels_map
+  | _ => idtac
+  end.
+  1: wp_bind (@! labels.Everything #())%E.
+  1: wp_apply (wp_Everything with "[$]").
+  1: iIntros (converted) "#Hconverted".
+  1: wp_auto.
+  1: iApply "HΦ".
+  1: iSplitR "Hconverted".
+  1: iCombineNamed "Hselector_field_*" as "Hselector_fields".
+  1: iAssert (typed_pointsto_def selector_l selector_c dq)
+    with "[Hselector_fields]" as "Hselector_l".
+  1: { iNamed "Hselector_fields". simpl. rewrite /named.
+       iFrame. }
+  1: iDestruct (struct_fields_combine (V:=v1.LabelSelector.t)
+    selector_l selector_c dq Hselector_nonnull with "Hselector_l") as
+    "Hselector_l".
+  1: iExists selector_c.
+  1: iFrame "Hselector_l".
+  1: rewrite /LabelSelectorV.deepown /named Hlabels_opt
+    Hexpressions_opt /=.
+  1: iFrame.
+  1: iFrame "%".
+  1: done.
+  1: assert (∀ labels_set, everything_matches labels_set ↔
+      LabelSelectorV.matches selector labels_set) as Hmatches.
+  1: { intros labels_set. symmetry. apply label_selector_matches_empty.
+       rewrite /LabelSelectorV.empty /LabelSelectorV.match_expressions_list
+         Hlabels_opt Hexpressions_opt /=.
+       split; [auto|done]. }
+  1: iPoseProof (is_selector_ext converted everything_matches
+    (LabelSelectorV.matches selector) Hmatches with "Hconverted") as
+    "Hconverted'".
+  1: (iExactEq "Hconverted'"; done).
+  1: wp_apply (wp_map_len_resolved (K:=go_string) (V:=go_string)
+    go.string go.string with "Hlabels_map").
+  1: iIntros "Hlabels_map".
+  1: wp_auto.
+  1: wp_apply (wp_slice_make3 (V:=labels.Requirement.t)
+    (t:=labels.Requirement)); first word.
+  1: iIntros (requirements_sl) "(Hrequirements & Hrequirements_cap & %)".
+  1: wp_auto.
+  1: set P := (λ (keys : list go_string) (i : Z),
+    ∃ (last_value last_key : go_string) (current_sl : slice.t)
+      (entries : list (labels.Requirement.t * LabelRequirementV.t)),
+      "Hv" ∷ v_ptr ↦ last_value ∗
+      "Hk" ∷ k_ptr ↦ last_key ∗
+      "Hrequirements_ptr" ∷ requirements_ptr ↦ current_sl ∗
+      "Hrequirements" ∷ current_sl ↦* (fst <$> entries) ∗
+      "Hrequirements_cap" ∷
+        own_slice_cap labels.Requirement.t current_sl (DfracOwn 1) ∗
+      "Hentries" ∷ ([∗ list] entry ∈ entries,
+        label_requirement_rep entry.1 entry.2) ∗
+      "%Hentries_pure" ∷ ⌜ snd <$> entries =
+        map_requirements (take (Z.to_nat i) keys) labels_map ⌝)%I.
+  1: wp_apply (wp_map_for_range_return_func
+    (key_type:=go.string) P with "Hlabels_map"); first done.
+  1: iIntros (keys) "%Hkeys".
+  1: destruct Hkeys as (Hkeys_dom & Hkeys_len & Hkeys_nodup).
+  1: iSplitL "v k requirements Hrequirements Hrequirements_cap".
+  1: { iExists ""%go, ""%go, requirements_sl, [].
+       rewrite /P fmap_nil take_0 /=.
+       iFrame. done. }
+  1: iSplitL "".
+  1: { iModIntro. iIntros (i key value) "%Hiter Hloop".
+       destruct Hiter as (Hi_bounds & Hkey_lookup & Hvalue_lookup).
+       iDestruct "Hloop" as
+         (last_value last_key current_sl entries)
+         "(Hv & Hk & Hrequirements_ptr & Hrequirements &
+          Hrequirements_cap & #Hentries & %Hentries_pure)".
+       simpl subst'.
+       wp_auto.
+       wp_apply wp_slice_literal. iSplitR; first done.
+       iIntros (value_sl) "[Hvalue_sl _]". wp_auto.
+       assert (valid_label_name key ∧ valid_label_value value)
+         as [Hkey_valid Hvalue_valid].
+       { apply Hlabels_valid. exact Hvalue_lookup. }
+       wp_apply (wp_NewRequirement with
+         "[$Hlabels_init $Hvalue_sl]").
+       { rewrite /valid_requirement_inputs /=.
+         split_and!; try done.
+         - constructor; [done|constructor].
+         - right. left. done. }
+       iIntros (requirement_l requirement_c)
+         "(Hrequirement_l & #Hrequirement)".
+       wp_auto.
+       wp_apply wp_slice_literal. iSplitR; first done.
+       iIntros (one_sl) "[Hone_sl _]". wp_auto.
+       wp_apply (wp_slice_append with
+         "[$Hrequirements $Hrequirements_cap $Hone_sl]").
+       iIntros (current_sl')
+         "(Hrequirements & Hrequirements_cap & Hone_sl)".
+       wp_auto.
+       iEval (simpl) in "Hrequirements".
+       iEval (simpl) in "Hrequirement".
+       iRight. iSplit; first done.
+       iExists value, key, current_sl',
+         (entries ++ [(requirement_c, map_label_requirement key value)]).
+       iFrame.
+       iSplit.
+       { assert (<[sint.nat (W64 0):=requirement_c]>
+             [(zero_val labels.Requirement.t)] = [requirement_c]) as Hone.
+         { simpl. done. }
+         iEval (rewrite Hone) in "Hrequirements".
+         iExactEq "Hrequirements".
+         rewrite /named. f_equal. rewrite fmap_app /=. done. }
+       iSplit.
+       { rewrite big_sepL_snoc /=.
+         iFrame "#". }
+       iPureIntro.
+       rewrite fmap_app /= Hentries_pure.
+       replace (Z.to_nat (i + 1)) with (S (Z.to_nat i)) by lia.
+       rewrite (take_S_r _ _ _ Hkey_lookup).
+       symmetry. apply map_requirements_snoc. exact Hvalue_lookup. }
+  1: iIntros "Hlabels_map Hloop".
+  1: iDestruct "Hloop" as
+    (last_value last_key map_requirements_sl map_entries)
+    "(Hv & Hk & Hrequirements_ptr & Hrequirements &
+     Hrequirements_cap & #Hmap_entries & %Hmap_entries_pure)".
+  1: assert (snd <$> map_entries = map_requirements keys labels_map)
+    as Hmap_entries_pure_all.
+  1: { rewrite Hmap_entries_pure.
+       replace (Z.to_nat (Z.of_nat (size labels_map))) with
+         (length keys) by lia.
+       assert (take (length keys) keys = keys) as Htake.
+       { apply take_ge. lia. }
+       rewrite Htake. done. }
+  1: wp_auto.
+  1: set I := (∃ (loop_i : w64)
+      (current_expression_c : v1.LabelSelectorRequirement.t)
+      (current_sl : slice.t)
+      (expression_entries :
+        list (labels.Requirement.t * LabelRequirementV.t)),
+      i_ptr ↦ loop_i ∗
+      expr_ptr ↦ current_expression_c ∗
+      requirements_ptr ↦ current_sl ∗
+      current_sl ↦* (fst <$> (map_entries ++ expression_entries)) ∗
+      own_slice_cap labels.Requirement.t current_sl (DfracOwn 1) ∗
+      ([∗ list] entry ∈ expression_entries,
+        label_requirement_rep entry.1 entry.2) ∗
+      v1.LabelSelector.MatchExpressions' selector_c ↦* expressions_c ∗
+      ([∗ list] c;expression ∈ expressions_c;expressions,
+        LabelSelectorRequirementV.deepown c expression dq) ∗
+      ⌜ Forall2 expression_converts
+          (take (sint.nat loop_i) expressions)
+          (snd <$> expression_entries) ⌝ ∗
+      ⌜ 0 ≤ sint.Z loop_i ≤ length expressions ⌝)%I.
+  1: iAssert I with
+    "[i expr Hrequirements_ptr Hrequirements Hrequirements_cap
+      Hexpressions_sl Hexpressions]" as "Hloop".
+  1: { iExists (W64 0), (zero_val v1.LabelSelectorRequirement.t),
+         map_requirements_sl, [].
+       rewrite fmap_app /= app_nil_r take_0.
+       iFrame.
+       iPureIntro. split; [constructor|word]. }
+  1: wp_for "Hloop".
+  1: iDestruct "Hloop" as
+    "(Hi & Hexpr_ptr & Hrequirements_ptr & Hrequirements &
+     Hrequirements_cap & #Hexpression_entries & Hexpressions_sl &
+     Hexpressions & %Hexpression_entries_pure & %Hloop_bounds)".
+  1: wp_auto.
+  1: wp_if_destruct.
+  1: destruct Hloop_bounds as [Hloop_nonnegative Hloop_upper].
+  1: assert (0 ≤ sint.Z loop_i < length expressions) as Hloop_lt by word.
+  1: list_elem expressions_c (sint.Z loop_i) as expression_c.
+  1: list_elem expressions (sint.Z loop_i) as expression.
+  1: assert (0 ≤ sint.Z loop_i <
+      sint.Z (slice.len (v1.LabelSelector.MatchExpressions' selector_c)))
+    as Hslice_bounds by word.
+  1: wp_pures.
+  1: rewrite decide_True; try exact Hslice_bounds.
+  1: wp_apply (wp_load_slice_index with "[$Hexpressions_sl]");
+    [word|iPureIntro; exact Hexpression_c_lookup|].
+  1: iIntros "Hexpressions_sl".
+  1: wp_auto.
+  1: iDestruct (big_sepL2_lookup_acc with "Hexpressions") as
+    "[Hexpression Hrestore_expressions]";
+    [exact Hexpression_c_lookup|exact Hexpression_lookup|].
+  1: iNamedPrefix "Hexpression" "Hexpression_".
+  1: assert (LabelSelectorRequirementV.valid expression)
+    as Hexpression_valid.
+  1: { rewrite Forall_forall in Hexpressions_valid.
+       apply Hexpressions_valid.
+       rewrite <-list_elem_of_In.
+       eapply list_elem_of_lookup_2. exact Hexpression_lookup. }
+  1: pose proof Hexpression_valid as Hvalid_expression.
+  1: destruct Hexpression_valid as
+    (Hoperator & Hin_values & Hexists_values & Hkey_valid & Hvalues_valid).
+  1: destruct Hoperator as
+    [Hoperator|[Hoperator|[Hoperator|Hoperator]]].
+  all: try (rewrite Hexpression_Hdeepown_operator Hoperator; wp_auto).
+  all: try lazymatch goal with
+  | Hoperator : LabelSelectorRequirementV.Operator' ?expression = _ |- _ =>
+      destruct expression.(LabelSelectorRequirementV.Values') as [values|]
+        eqn:Hvalues_opt
+  end.
+  all: try lazymatch goal with
+  | Hvalues_opt : LabelSelectorRequirementV.Values' ?expression = Some ?values
+      |- _ =>
+      iRename "Hexpression_Hdeepown_values_some" into "Hsource_values";
+      rewrite /LabelSelectorRequirementV.values_list Hvalues_opt /=
+        in Hvalues_valid Hin_values Hexists_values
+  | Hvalues_opt : LabelSelectorRequirementV.Values' ?expression = None
+      |- _ =>
+      rewrite /LabelSelectorRequirementV.values_list Hvalues_opt /=
+        in Hvalues_valid Hin_values Hexists_values
+  end.
+  1: iPoseProof (own_slice_nil (V:=go_string) (DfracOwn 1))
+    as "Hcopied_values".
+  1: iPoseProof (own_slice_cap_nil (V:=go_string))
+    as "Hcopied_values_cap".
+  1: wp_apply (wp_slice_append (V:=go_string) (t:=go.string)
+    (st:=go.SliceType go.string)
+    slice.nil [] (v1.LabelSelectorRequirement.Values' expression_c)
+    values dq with
+    "[$Hcopied_values $Hcopied_values_cap $Hsource_values]").
+  1: iIntros (copied_values_sl)
+    "(Hcopied_values_out & Hcopied_values_cap_out & Hsource_values_out)".
+  1: iEval (simpl) in "Hcopied_values_out".
+  1: wp_auto.
+  1: rewrite Hexpression_Hdeepown_key.
+  1: wp_apply (wp_NewRequirement with
+    "[$Hlabels_init $Hcopied_values_out]").
+  1: { rewrite /valid_requirement_inputs /=.
+       split_and!; try done.
+       left. split; [left; done|].
+       apply Hin_values. left. exact Hoperator. }
+  1: iIntros (requirement_l requirement_c')
+    "(Hrequirement_l & #Hrequirement)".
+  1: wp_auto.
+  1: wp_apply wp_slice_literal.
+  1: iSplitR; first done.
+  1: iIntros (one_requirement_l) "[Hone_requirement _]".
+  1: wp_auto.
+  1: wp_apply (wp_slice_append with
+    "[$Hrequirements $Hrequirements_cap $Hone_requirement]").
+  1: iIntros (current_sl')
+    "(Hrequirements_out & Hrequirements_cap_out & Hone_requirement_out)".
+  1: wp_auto.
+  1: set (new_requirement := LabelRequirementV.mk
+    expression.(LabelSelectorRequirementV.Key') "in"%go values).
+  1: assert (expression_converts expression new_requirement)
+    as Hexpression_converts.
+  1: { rewrite /expression_converts /new_requirement /= Hoperator
+         /LabelSelectorRequirementV.values_list Hvalues_opt /=.
+       tauto. }
+  1: iAssert (LabelSelectorRequirementV.deepown expression_c expression dq)
+    with "[Hsource_values_out]" as "Hexpression".
+  1: { rewrite /LabelSelectorRequirementV.deepown /named Hvalues_opt /=.
+       iFrame. iPureIntro. split_and!; done. }
+  1: iSpecialize ("Hrestore_expressions" with "Hexpression").
+  1: assert (<[sint.nat (W64 0):=requirement_c']>
+      [(zero_val labels.Requirement.t)] = [requirement_c'])
+    as Hone_requirement.
+  1: { simpl. done. }
+  1: iEval (rewrite Hone_requirement) in "Hrequirements_out".
+  1: iApply wp_for_post_do.
+  1: wp_auto.
+  1: iFrame "HΦ Hselector_field_MatchLabels
+    Hselector_field_MatchExpressions Hlabels_map Hv Hk".
+  1: iExists (word.add loop_i (W64 1)), expression_c, current_sl',
+    (expression_entries ++ [(requirement_c', new_requirement)]).
+  1: iFrame "Hi Hexpr_ptr Hrequirements_ptr Hrequirements_cap_out
+    Hexpressions_sl Hrestore_expressions".
+  1: iSplitL "Hrequirements_out".
+  1: { iExactEq "Hrequirements_out".
+       f_equal. rewrite !fmap_app /=. symmetry. apply app_assoc. }
+  1: iSplit.
+  1: { rewrite big_sepL_snoc /=. iFrame "#". }
+  1: iSplit; first iFrame.
+  1: iPureIntro.
+  1: replace (sint.nat (word.add loop_i (W64 1))) with
+    (S (sint.nat loop_i)) by word.
+  1: rewrite (take_S_r _ _ _ Hexpression_lookup) fmap_app /=.
+  1: apply Forall2_app; [exact Hexpression_entries_pure|].
+  1: constructor; [exact Hexpression_converts|constructor].
+  1: word.
+  1: (exfalso; apply (Hin_values (or_introl Hoperator))).
+  1: done.
+
+  Ltac finish_expression mapped_operator values source_sl frac valid_expression :=
+    let copied_values_sl := fresh "copied_values_sl" in
+    let requirement_l := fresh "requirement_l" in
+    let requirement_c := fresh "requirement_c" in
+    let one_requirement_l := fresh "one_requirement_l" in
+    let current_sl_next := fresh "current_sl" in
+    let values_nil := fresh "Hvalues_nil" in
+    lazymatch goal with
+    | Hvalues_opt : LabelSelectorRequirementV.Values' ?expression = _,
+      Hexpression_Hdeepown_values_none :
+        v1.LabelSelectorRequirement.Values' ?expression_c = slice.nil ↔ _,
+      Hexpression_Hdeepown_key :
+        v1.LabelSelectorRequirement.Key' ?expression_c = _,
+      Hoperator : LabelSelectorRequirementV.Operator' ?expression = _,
+      Hin_values : _, Hexists_values : _, Hkey_valid : _,
+      Hvalues_valid : _,
+      Hexpression_entries_pure :
+        Forall2 expression_converts (take (sint.nat ?loop_i) ?expressions)
+          (snd <$> ?expression_entries),
+      Hexpression_lookup : ?expressions !! sint.nat ?loop_i = Some ?expression
+      |- _ =>
+    lazymatch type of Hvalues_opt with
+    | LabelSelectorRequirementV.Values' expression = None =>
+        assert (v1.LabelSelectorRequirement.Values' expression_c = slice.nil)
+          as values_nil;
+        [apply (proj2 Hexpression_Hdeepown_values_none); done|];
+        rewrite values_nil;
+        iAssert (slice.nil ↦*{frac} ([] : list go_string))%I
+          as "Hsource_values";
+        [iApply own_slice_nil|]
+    | _ => idtac
+    end;
+    set (new_requirement := LabelRequirementV.mk
+      expression.(LabelSelectorRequirementV.Key') mapped_operator values);
+    assert (expression_converts expression new_requirement)
+      as Hexpression_converts;
+    [rewrite /expression_converts /new_requirement /= Hoperator
+       /LabelSelectorRequirementV.values_list Hvalues_opt /=;
+     split; [done|]; split; [done|];
+     first [left; split; done
+       | right; left; split; done
+       | right; right; left; split; done
+       | right; right; right; split; done]|];
+    pose proof (expression_converts_valid_inputs _ _ valid_expression
+      Hexpression_converts) as Hvalid_inputs;
+    iPoseProof (own_slice_nil (V:=go_string) (DfracOwn 1))
+      as "Hcopied_values";
+    iPoseProof (own_slice_cap_nil (V:=go_string))
+      as "Hcopied_values_cap";
+    iAssert (slice.nil ↦* ([] : list go_string) ∗
+      own_slice_cap go_string slice.nil (DfracOwn 1) ∗
+      source_sl ↦*{frac} values)%I
+      with "[Hcopied_values Hcopied_values_cap Hsource_values]"
+      as "Happend_values";
+    [iSplitL "Hcopied_values"; [iExact "Hcopied_values"|];
+     iSplitL "Hcopied_values_cap"; [iExact "Hcopied_values_cap"|];
+     lazymatch type of Hvalues_opt with
+     | LabelSelectorRequirementV.Values' expression = None =>
+         iExact "Hsource_values"
+     | _ => iExact "Hsource_values"
+     end|];
+    wp_apply (wp_slice_append (V:=go_string) (t:=go.string)
+      (st:=go.SliceType go.string)
+      slice.nil [] source_sl
+      values frac with "Happend_values");
+    iIntros (copied_values_sl)
+      "(Hcopied_values_out & Hcopied_values_cap_out & Hsource_values_out)";
+    iEval (simpl) in "Hcopied_values_out";
+    wp_auto;
+    rewrite Hexpression_Hdeepown_key;
+    wp_apply (wp_NewRequirement with
+      "[$Hlabels_init $Hcopied_values_out]");
+    [exact Hvalid_inputs|];
+    iIntros (requirement_l requirement_c)
+      "(Hrequirement_l & #Hrequirement)";
+    wp_auto;
+    wp_apply wp_slice_literal;
+    iSplitR; [done|];
+    iIntros (one_requirement_l) "[Hone_requirement _]";
+    wp_auto;
+    wp_apply (wp_slice_append with
+      "[$Hrequirements $Hrequirements_cap $Hone_requirement]");
+    iIntros (current_sl_next)
+      "(Hrequirements_out & Hrequirements_cap_out & Hone_requirement_out)";
+    wp_auto;
+    iAssert (LabelSelectorRequirementV.deepown expression_c expression frac)
+      with "[Hsource_values_out]" as "Hexpression";
+    [rewrite /LabelSelectorRequirementV.deepown /named Hvalues_opt /=;
+     iFrame; iPureIntro; split_and!; done|];
+    iSpecialize ("Hrestore_expressions" with "Hexpression");
+    assert (<[sint.nat (W64 0):=requirement_c]>
+        [(zero_val labels.Requirement.t)] = [requirement_c])
+      as Hone_requirement;
+    [simpl; done|];
+    iEval (rewrite Hone_requirement) in "Hrequirements_out";
+    iApply wp_for_post_do;
+    wp_auto;
+    iFrame "HΦ Hselector_field_MatchLabels
+      Hselector_field_MatchExpressions";
+    try iFrame "Hv";
+    try iFrame "Hk";
+    try iFrame "Hlabels_map";
+    iExists (word.add loop_i (W64 1)), expression_c, current_sl_next,
+      (expression_entries ++ [(requirement_c, new_requirement)]);
+    iFrame "Hi Hexpr_ptr Hrequirements_ptr Hrequirements_cap_out
+      Hexpressions_sl Hrestore_expressions";
+    iSplitL "Hrequirements_out";
+    [iExactEq "Hrequirements_out";
+     f_equal; rewrite !fmap_app /=;
+     first [done | (symmetry; apply app_assoc)]|];
+    iSplit;
+    [rewrite big_sepL_snoc /=; iFrame "#"|];
+    iSplit; [iFrame|];
+    iPureIntro;
+    [replace (sint.nat (word.add loop_i (W64 1))) with
+       (S (sint.nat loop_i)) by word;
+     rewrite (take_S_r _ _ _ Hexpression_lookup) fmap_app /=;
+     apply Forall2_app;
+     [exact Hexpression_entries_pure|];
+     constructor;
+     [exact Hexpression_converts|constructor]
+    |word]
+    end.
+
+  1: finish_expression "notin"%go values
+    (v1.LabelSelectorRequirement.Values' expression_c) dq Hvalid_expression.
+  1: (exfalso; apply (Hin_values (or_intror Hoperator))).
+  1: done.
+  1: finish_expression "exists"%go values
+    (v1.LabelSelectorRequirement.Values' expression_c) dq Hvalid_expression.
+  1: finish_expression "exists"%go ([] : list go_string) slice.nil dq
+    Hvalid_expression.
+  1: finish_expression "!"%go values
+    (v1.LabelSelectorRequirement.Values' expression_c) dq Hvalid_expression.
+  1: finish_expression "!"%go ([] : list go_string) slice.nil dq
+    Hvalid_expression.
+
+  1: assert (sint.nat loop_i = length expressions) as Hloop_done by word.
+  1: assert (take (sint.nat loop_i) expressions = expressions) as Htake_all.
+  1: { apply take_ge. lia. }
+  1: rewrite Htake_all in Hexpression_entries_pure.
+  1: assert (length (map_requirements keys labels_map) = length keys)
+    as Hmap_requirements_len.
+  1: { apply map_requirements_length. intros key Hkey.
+       assert (key ∈ dom labels_map) as Hkey_dom.
+       { rewrite <- list_elem_of_In in Hkey.
+         rewrite <- Hkeys_dom. rewrite elem_of_list_to_set. exact Hkey. }
+       rewrite elem_of_dom in Hkey_dom. exact Hkey_dom. }
+  1: pose proof (f_equal (@length LabelRequirementV.t)
+    Hmap_entries_pure_all) as Hmap_entries_len.
+  1: rewrite !length_fmap Hmap_requirements_len Hkeys_len
+    in Hmap_entries_len.
+  1: pose proof (Forall2_length Hexpression_entries_pure)
+    as Hexpression_entries_len.
+  1: rewrite length_fmap in Hexpression_entries_len.
+  1: assert (Forall LabelRequirementV.supported
+      (snd <$> (map_entries ++ expression_entries))) as Hsupported.
+  1: { rewrite fmap_app. apply Forall_app. split.
+       - rewrite Hmap_entries_pure_all. apply map_requirements_supported.
+       - eapply expression_conversions_supported.
+         exact Hexpression_entries_pure. }
+  1: assert (Z.of_nat (length (map_entries ++ expression_entries)) ≤
+      2 ^ 63 - 1) as Hentries_size.
+  1: { rewrite length_app Hmap_entries_len.
+       rewrite <- Hexpression_entries_len. lia. }
+  1: iAssert (by_key_contents current_sl
+      (map_entries ++ expression_entries))
+    with "[Hrequirements Hmap_entries Hexpression_entries]"
+    as "Hrequirements_contents".
+  1: { rewrite /by_key_contents big_sepL_app.
+       iFrame "Hrequirements". iFrame "#". }
+  1: wp_apply wp_NewSelector.
+  1: iIntros (empty_selector) "[%Hempty_selector #Hempty_selector_rep]".
+  1: rewrite Hempty_selector.
+  1: wp_auto.
+  1: wp_apply (wp_empty_internalSelector__Add current_sl
+    (map_entries ++ expression_entries)
+    with "[$Hlabels_init $Hrequirements_contents]"); first exact Hentries_size.
+  1: exact Hsupported.
+  1: iIntros (converted) "#Hconverted".
+  1: wp_auto.
+  1: iApply "HΦ".
+  1: iSplitR "Hconverted".
+  1: iCombineNamed "Hselector_field_*" as "Hselector_fields".
+  1: iAssert (typed_pointsto_def selector_l selector_c dq)
+    with "[Hselector_fields]" as "Hselector_l".
+  1: { iNamed "Hselector_fields". simpl. rewrite /named.
+       iFrame; try done. }
+  1: iDestruct (struct_fields_combine (V:=v1.LabelSelector.t)
+    selector_l selector_c dq Hselector_nonnull with "Hselector_l") as
+    "Hselector_l".
+  1: iExists selector_c.
+  1: iFrame "Hselector_l".
+  1: rewrite /LabelSelectorV.deepown /named Hlabels_opt
+    Hexpressions_opt /=.
+  1: iFrame.
+  1: iFrame "%".
+  1: done.
+  1: assert (∀ labels_set,
+      selector_matches (snd <$> (map_entries ++ expression_entries))
+        labels_set ↔ LabelSelectorV.matches selector labels_set)
+    as Hmatches.
+  1: { intros labels_set.
+       rewrite fmap_app Hmap_entries_pure_all /selector_matches Forall_app.
+       change ((selector_matches (map_requirements keys labels_map)
+           labels_set ∧
+         selector_matches (snd <$> expression_entries) labels_set) ↔
+         LabelSelectorV.matches selector labels_set).
+       rewrite (map_requirements_match keys labels_map labels_set Hkeys_dom).
+       rewrite (expression_conversions_match expressions
+         (snd <$> expression_entries) labels_set
+         Hexpression_entries_pure).
+       rewrite /LabelSelectorV.matches
+         /LabelSelectorV.match_expressions_list Hlabels_opt
+         Hexpressions_opt /=. done. }
+  1: iPoseProof (is_selector_ext converted
+    (selector_matches (snd <$> (map_entries ++ expression_entries)))
+    (LabelSelectorV.matches selector) Hmatches with "Hconverted") as
+    "Hconverted'".
+  1: iExact "Hconverted'".
+
+  1: wp_bind (@! labels.Everything #())%E.
+  1: wp_apply (wp_Everything with "[$]").
+  1: iIntros (converted) "#Hconverted".
+  1: wp_auto.
+  1: iApply "HΦ".
+  1: iSplitR "Hconverted".
+  1: iCombineNamed "Hselector_field_*" as "Hselector_fields".
+  1: iAssert (typed_pointsto_def selector_l selector_c dq)
+    with "[Hselector_fields]" as "Hselector_l".
+  1: { iNamed "Hselector_fields". simpl. rewrite /named.
+       iFrame; try done. }
+  1: iDestruct (struct_fields_combine (V:=v1.LabelSelector.t)
+    selector_l selector_c dq Hselector_nonnull with "Hselector_l") as
+    "Hselector_l".
+  1: iExists selector_c.
+  1: iFrame "Hselector_l".
+  1: rewrite /LabelSelectorV.deepown /named Hlabels_opt
+    Hexpressions_opt /=.
+  1: iFrame.
+  1: iFrame "%".
+  1: done.
+  1: assert (∀ labels_set, everything_matches labels_set ↔
+      LabelSelectorV.matches selector labels_set) as Hmatches.
+  1: { intros labels_set. symmetry. apply label_selector_matches_empty.
+       rewrite /LabelSelectorV.empty /LabelSelectorV.match_expressions_list
+         Hlabels_opt Hexpressions_opt /=. split; [auto|done]. }
+  1: iPoseProof (is_selector_ext converted everything_matches
+    (LabelSelectorV.matches selector) Hmatches with "Hconverted") as
+    "Hconverted'".
+  1: iExact "Hconverted'".
+
+  1: wp_apply (wp_map_len_resolved (K:=go_string) (V:=go_string)
+    go.string go.string with "Hlabels_map").
+  1: iIntros "Hlabels_map".
+  1: wp_auto.
+  1: unfold expressions in Hexpressions_word_len.
+  1: simpl in Hexpressions_word_len.
+  1: wp_apply (wp_slice_make3 (V:=labels.Requirement.t)
+    (t:=labels.Requirement)); first word.
+  1: iIntros (requirements_sl) "(Hrequirements & Hrequirements_cap & %)".
+  1: wp_auto.
+  1: set P := (λ (keys : list go_string) (i : Z),
+    ∃ (last_value last_key : go_string) (current_sl : slice.t)
+      (entries : list (labels.Requirement.t * LabelRequirementV.t)),
+      "Hv" ∷ v_ptr ↦ last_value ∗
+      "Hk" ∷ k_ptr ↦ last_key ∗
+      "Hrequirements_ptr" ∷ requirements_ptr ↦ current_sl ∗
+      "Hrequirements" ∷ current_sl ↦* (fst <$> entries) ∗
+      "Hrequirements_cap" ∷
+        own_slice_cap labels.Requirement.t current_sl (DfracOwn 1) ∗
+      "Hentries" ∷ ([∗ list] entry ∈ entries,
+        label_requirement_rep entry.1 entry.2) ∗
+      "%Hentries_pure" ∷ ⌜ snd <$> entries =
+        map_requirements (take (Z.to_nat i) keys) labels_map ⌝)%I.
+  1: wp_apply (wp_map_for_range_return_func
+    (key_type:=go.string) P with "Hlabels_map"); first done.
+  1: iIntros (keys) "%Hkeys".
+  1: destruct Hkeys as (Hkeys_dom & Hkeys_len & Hkeys_nodup).
+  1: iSplitL "v k requirements Hrequirements Hrequirements_cap".
+  1: { iExists ""%go, ""%go, requirements_sl, [].
+       rewrite /P fmap_nil take_0 /=. iFrame. done. }
+  1: iSplitL "".
+  1: { iModIntro. iIntros (i key value) "%Hiter Hloop".
+       destruct Hiter as (Hi_bounds & Hkey_lookup & Hvalue_lookup).
+       iDestruct "Hloop" as
+         (last_value last_key current_sl entries)
+         "(Hv & Hk & Hrequirements_ptr & Hrequirements &
+          Hrequirements_cap & #Hentries & %Hentries_pure)".
+       simpl subst'. wp_auto.
+       wp_apply wp_slice_literal. iSplitR; first done.
+       iIntros (value_sl) "[Hvalue_sl _]". wp_auto.
+       assert (valid_label_name key ∧ valid_label_value value)
+         as [Hkey_valid Hvalue_valid].
+       { apply Hlabels_valid. exact Hvalue_lookup. }
+       wp_apply (wp_NewRequirement with
+         "[$Hlabels_init $Hvalue_sl]").
+       { rewrite /valid_requirement_inputs /=.
+         split_and!; try done.
+         - constructor; [done|constructor].
+         - right. left. done. }
+       iIntros (requirement_l requirement_c)
+         "(Hrequirement_l & #Hrequirement)".
+       wp_auto.
+       wp_apply wp_slice_literal. iSplitR; first done.
+       iIntros (one_sl) "[Hone_sl _]". wp_auto.
+       wp_apply (wp_slice_append with
+         "[$Hrequirements $Hrequirements_cap $Hone_sl]").
+       iIntros (current_sl')
+         "(Hrequirements & Hrequirements_cap & Hone_sl)".
+       wp_auto.
+       iEval (simpl) in "Hrequirements".
+       iEval (simpl) in "Hrequirement".
+       iRight. iSplit; first done.
+       iExists value, key, current_sl',
+         (entries ++ [(requirement_c, map_label_requirement key value)]).
+       iFrame.
+       iSplit.
+       { assert (<[sint.nat (W64 0):=requirement_c]>
+             [(zero_val labels.Requirement.t)] = [requirement_c]) as Hone.
+         { simpl. done. }
+         iEval (rewrite Hone) in "Hrequirements".
+         iExactEq "Hrequirements".
+         rewrite /named. f_equal. rewrite fmap_app /=. done. }
+       iSplit.
+       { rewrite big_sepL_snoc /=. iFrame "#". }
+       iPureIntro.
+       rewrite fmap_app /= Hentries_pure.
+       replace (Z.to_nat (i + 1)) with (S (Z.to_nat i)) by lia.
+       rewrite (take_S_r _ _ _ Hkey_lookup).
+       symmetry. apply map_requirements_snoc. exact Hvalue_lookup. }
+  1: iIntros "Hlabels_map Hloop".
+  1: iDestruct "Hloop" as
+    (last_value last_key map_requirements_sl map_entries)
+    "(Hv & Hk & Hrequirements_ptr & Hrequirements &
+     Hrequirements_cap & #Hmap_entries & %Hmap_entries_pure)".
+  1: assert (snd <$> map_entries = map_requirements keys labels_map)
+    as Hmap_entries_pure_all.
+  1: { rewrite Hmap_entries_pure.
+       replace (Z.to_nat (Z.of_nat (size labels_map))) with
+         (length keys) by lia.
+       assert (take (length keys) keys = keys) as Htake.
+       { apply take_ge. lia. }
+       rewrite Htake. done. }
+  1: wp_auto.
+  1: set I := (∃ (loop_i : w64)
+      (current_expression_c : v1.LabelSelectorRequirement.t)
+      (current_sl : slice.t)
+      (expression_entries :
+        list (labels.Requirement.t * LabelRequirementV.t)),
+      i_ptr ↦ loop_i ∗
+      expr_ptr ↦ current_expression_c ∗
+      requirements_ptr ↦ current_sl ∗
+      current_sl ↦* (fst <$> (map_entries ++ expression_entries)) ∗
+      own_slice_cap labels.Requirement.t current_sl (DfracOwn 1) ∗
+      ([∗ list] entry ∈ expression_entries,
+        label_requirement_rep entry.1 entry.2) ∗
+      v1.LabelSelector.MatchExpressions' selector_c ↦* expressions_c ∗
+      ([∗ list] c;expression ∈ expressions_c;expressions,
+        LabelSelectorRequirementV.deepown c expression dq) ∗
+      ⌜ Forall2 expression_converts
+          (take (sint.nat loop_i) expressions)
+          (snd <$> expression_entries) ⌝ ∗
+      ⌜ 0 ≤ sint.Z loop_i ≤ length expressions ⌝)%I.
+  1: iAssert I with
+    "[i expr Hrequirements_ptr Hrequirements Hrequirements_cap
+      Hexpressions_sl Hexpressions]" as "Hloop".
+  1: { iExists (W64 0), (zero_val v1.LabelSelectorRequirement.t),
+         map_requirements_sl, [].
+       rewrite fmap_app /= app_nil_r take_0.
+       unfold expressions, expressions_c. simpl.
+       iFrame "i expr Hrequirements_ptr Hrequirements Hrequirements_cap
+         Hexpressions_sl".
+       all: done. }
+  1: try iClear "Hexpressions_sl Hexpressions".
+  1: wp_for "Hloop".
+  1: iDestruct "Hloop" as
+    "(Hi & Hexpr_ptr & Hrequirements_ptr & Hrequirements &
+     Hrequirements_cap & #Hexpression_entries & Hexpressions_sl &
+     Hexpressions & %Hexpression_entries_pure & %Hloop_bounds)".
+  1: wp_auto.
+  1: wp_if_destruct.
+  1: exfalso; word.
+  1: unfold expressions in Hexpression_entries_pure.
+  1: rewrite take_nil in Hexpression_entries_pure.
+  1: assert (expression_entries = []) as ->.
+  1: { apply (fmap_eq_nil snd).
+       eapply Forall2_nil_left. exact Hexpression_entries_pure. }
+  1: assert (snd <$> map_entries = map_requirements keys labels_map)
+    as Hmap_entries_all by exact Hmap_entries_pure_all.
+  1: assert (length (map_requirements keys labels_map) = length keys)
+    as Hmap_requirements_len.
+  1: { apply map_requirements_length. intros key Hkey.
+       rewrite <- list_elem_of_In in Hkey.
+       assert (key ∈ dom labels_map) as Hkey_dom.
+       { rewrite <- Hkeys_dom. rewrite elem_of_list_to_set. exact Hkey. }
+       rewrite elem_of_dom in Hkey_dom. exact Hkey_dom. }
+  1: pose proof (f_equal (@length LabelRequirementV.t)
+    Hmap_entries_all) as Hmap_entries_len.
+  1: rewrite !length_fmap Hmap_requirements_len Hkeys_len
+    in Hmap_entries_len.
+  1: assert (Forall LabelRequirementV.supported (snd <$> map_entries))
+    as Hsupported by
+      (rewrite Hmap_entries_all; apply map_requirements_supported).
+  1: assert (Z.of_nat (length map_entries) ≤ 2 ^ 63 - 1)
+    as Hentries_size by (rewrite Hmap_entries_len; lia).
+  1: iEval (rewrite app_nil_r) in "Hrequirements".
+  1: iAssert (by_key_contents current_sl map_entries)
+    with "[Hrequirements Hmap_entries]" as "Hrequirements_contents".
+  1: { rewrite /by_key_contents. iFrame "Hrequirements". iFrame "#". }
+  1: wp_apply wp_NewSelector.
+  1: iIntros (empty_selector) "[%Hempty_selector #Hempty_selector_rep]".
+  1: rewrite Hempty_selector.
+  1: wp_auto.
+  1: wp_apply (wp_empty_internalSelector__Add current_sl map_entries
+    with "[$Hlabels_init $Hrequirements_contents]"); first exact Hentries_size.
+  1: exact Hsupported.
+  1: iIntros (converted) "#Hconverted".
+  1: wp_auto.
+  1: iApply "HΦ".
+  1: iSplitR "Hconverted".
+  1: iCombineNamed "Hselector_field_*" as "Hselector_fields".
+  1: iAssert (typed_pointsto_def selector_l selector_c dq)
+    with "[Hselector_fields]" as "Hselector_l".
+  1: { iNamed "Hselector_fields". simpl. rewrite /named.
+       iFrame; try done. }
+  1: iDestruct (struct_fields_combine (V:=v1.LabelSelector.t)
+    selector_l selector_c dq Hselector_nonnull with "Hselector_l") as
+    "Hselector_l".
+  1: iExists selector_c.
+  1: iFrame "Hselector_l".
+  1: rewrite /LabelSelectorV.deepown /named Hlabels_opt
+    Hexpressions_opt /=.
+  1: iFrame.
+  1: iFrame "%".
+  1: done.
+  1: assert (∀ labels_set, selector_matches (snd <$> map_entries) labels_set ↔
+      LabelSelectorV.matches selector labels_set) as Hmatches.
+  1: { intros labels_set. rewrite Hmap_entries_all.
+       rewrite (map_requirements_match keys labels_map labels_set Hkeys_dom).
+       rewrite /LabelSelectorV.matches
+         /LabelSelectorV.match_expressions_list Hlabels_opt
+         Hexpressions_opt /=.
+       split.
+       - intros Hmatch. split; [exact Hmatch|constructor].
+       - intros [Hmatch _]. exact Hmatch. }
+  1: iPoseProof (is_selector_ext converted
+    (selector_matches (snd <$> map_entries))
+    (LabelSelectorV.matches selector) Hmatches with "Hconverted") as
+    "Hconverted'".
+  1: iExact "Hconverted'".
+  all: wp_if_destruct.
+
+  1: assert (length expressions = 0%nat) as Hexpressions_empty by word.
+  1: apply nil_length_inv in Hexpressions_empty.
+  1: subst expressions.
+  1: wp_bind (@! labels.Everything #())%E.
+  1: wp_apply (wp_Everything with "[$]").
+  1: iIntros (converted) "#Hconverted".
+  1: wp_auto.
+  1: iApply "HΦ".
+  1: iSplitR "Hconverted".
+  1: iCombineNamed "Hselector_field_*" as "Hselector_fields".
+  1: iAssert (typed_pointsto_def selector_l selector_c dq)
+    with "[Hselector_fields]" as "Hselector_l".
+  1: { iNamed "Hselector_fields". simpl.
+       rewrite /named Hlabels_map_nil. iFrame. }
+  1: iDestruct (struct_fields_combine (V:=v1.LabelSelector.t)
+    selector_l selector_c dq Hselector_nonnull with "Hselector_l") as
+    "Hselector_l".
+  1: iExists selector_c.
+  1: iFrame "Hselector_l".
+  1: rewrite /LabelSelectorV.deepown /named Hlabels_opt
+    Hexpressions_opt /=.
+  1: iFrame.
+  1: iFrame "%".
+  1: assert (∀ labels_set, everything_matches labels_set ↔
+      LabelSelectorV.matches selector labels_set) as Hmatches.
+  1: { intros labels_set. symmetry. apply label_selector_matches_empty.
+       rewrite /LabelSelectorV.empty /LabelSelectorV.match_expressions_list
+         Hlabels_opt Hexpressions_opt /=. split; [auto|done]. }
+  1: iPoseProof (is_selector_ext converted everything_matches
+    (LabelSelectorV.matches selector) Hmatches with "Hconverted") as
+    "Hconverted'".
+  1: iExact "Hconverted'".
+
+  3: unfold expressions in Hexpressions_word_len.
+  3: simpl in Hexpressions_word_len.
+  3: exfalso; word.
+
+  2: wp_bind (@! labels.Everything #())%E.
+  2: wp_apply (wp_Everything with "[$]").
+  2: iIntros (converted) "#Hconverted".
+  2: wp_auto.
+  2: iApply "HΦ".
+  2: iSplitR "Hconverted".
+  2: iCombineNamed "Hselector_field_*" as "Hselector_fields".
+  2: iAssert (typed_pointsto_def selector_l selector_c dq)
+    with "[Hselector_fields]" as "Hselector_l".
+  2: { iNamed "Hselector_fields". simpl.
+       rewrite /named Hlabels_map_nil. iFrame. }
+  2: iDestruct (struct_fields_combine (V:=v1.LabelSelector.t)
+    selector_l selector_c dq Hselector_nonnull with "Hselector_l") as
+    "Hselector_l".
+  2: iExists selector_c.
+  2: iFrame "Hselector_l".
+  2: rewrite /LabelSelectorV.deepown /named Hlabels_opt
+    Hexpressions_opt /=.
+  2: iFrame.
+  2: iFrame "%".
+  2: assert (∀ labels_set, everything_matches labels_set ↔
+      LabelSelectorV.matches selector labels_set) as Hmatches.
+  2: { intros labels_set. symmetry. apply label_selector_matches_empty.
+       rewrite /LabelSelectorV.empty /LabelSelectorV.match_expressions_list
+         Hlabels_opt Hexpressions_opt /=. split; [auto|done]. }
+  2: iPoseProof (is_selector_ext converted everything_matches
+    (LabelSelectorV.matches selector) Hmatches with "Hconverted") as
+    "Hconverted'".
+  2: iExact "Hconverted'".
+
+  1: wp_apply (wp_map_len_nil_resolved (K:=go_string) (V:=go_string)
+    go.string go.string).
+  1: wp_pures.
+  1: wp_apply (wp_slice_make3 (V:=labels.Requirement.t)
+    (t:=labels.Requirement)); first word.
+  1: iIntros (requirements_sl) "(Hrequirements & Hrequirements_cap & %)".
+  1: wp_auto.
+  1: wp_apply (wp_map_for_range_nil go.string go.string).
+  1: wp_pures.
+  1: set I := (∃ (loop_i : w64)
+      (current_expression_c : v1.LabelSelectorRequirement.t)
+      (current_sl : slice.t)
+      (expression_entries :
+        list (labels.Requirement.t * LabelRequirementV.t)),
+      i_ptr ↦ loop_i ∗
+      expr_ptr ↦ current_expression_c ∗
+      requirements_ptr ↦ current_sl ∗
+      current_sl ↦* (fst <$> expression_entries) ∗
+      own_slice_cap labels.Requirement.t current_sl (DfracOwn 1) ∗
+      ([∗ list] entry ∈ expression_entries,
+        label_requirement_rep entry.1 entry.2) ∗
+      v1.LabelSelector.MatchExpressions' selector_c ↦* expressions_c ∗
+      ([∗ list] c;expression ∈ expressions_c;expressions,
+        LabelSelectorRequirementV.deepown c expression dq) ∗
+      ⌜ Forall2 expression_converts
+          (take (sint.nat loop_i) expressions)
+          (snd <$> expression_entries) ⌝ ∗
+      ⌜ 0 ≤ sint.Z loop_i ≤ length expressions ⌝)%I.
+  1: iAssert I with
+    "[i expr requirements Hrequirements Hrequirements_cap
+      Hexpressions_sl Hexpressions]" as "Hloop".
+  1: { iExists (W64 0), (zero_val v1.LabelSelectorRequirement.t),
+         requirements_sl, [].
+       rewrite take_0 /=.
+       iFrame. iPureIntro. split; [constructor|word]. }
+  1: wp_for "Hloop".
+  1: iDestruct "Hloop" as
+    "(Hi & Hexpr_ptr & Hrequirements_ptr & Hrequirements &
+     Hrequirements_cap & #Hexpression_entries & Hexpressions_sl &
+     Hexpressions & %Hexpression_entries_pure & %Hloop_bounds)".
+  1: wp_auto.
+  1: wp_if_destruct.
+  1: destruct Hloop_bounds as [Hloop_nonnegative Hloop_upper].
+  1: assert (0 ≤ sint.Z loop_i < length expressions) as Hloop_lt by word.
+  1: list_elem expressions_c (sint.Z loop_i) as expression_c.
+  1: list_elem expressions (sint.Z loop_i) as expression.
+  1: assert (0 ≤ sint.Z loop_i <
+      sint.Z (slice.len (v1.LabelSelector.MatchExpressions' selector_c)))
+    as Hslice_bounds by word.
+  1: wp_pures.
+  1: rewrite decide_True; try exact Hslice_bounds.
+  1: wp_apply (wp_load_slice_index with "[$Hexpressions_sl]");
+    [word|iPureIntro; exact Hexpression_c_lookup|].
+  1: iIntros "Hexpressions_sl".
+  1: wp_auto.
+  1: iDestruct (big_sepL2_lookup_acc with "Hexpressions") as
+    "[Hexpression Hrestore_expressions]";
+    [exact Hexpression_c_lookup|exact Hexpression_lookup|].
+  1: iNamedPrefix "Hexpression" "Hexpression_".
+  1: assert (LabelSelectorRequirementV.valid expression)
+    as Hexpression_valid.
+  1: { rewrite Forall_forall in Hexpressions_valid.
+       apply Hexpressions_valid.
+       rewrite <-list_elem_of_In.
+       eapply list_elem_of_lookup_2. exact Hexpression_lookup. }
+  1: pose proof Hexpression_valid as Hvalid_expression.
+  1: destruct Hexpression_valid as
+    (Hoperator & Hin_values & Hexists_values & Hkey_valid & Hvalues_valid).
+  1: destruct Hoperator as
+    [Hoperator|[Hoperator|[Hoperator|Hoperator]]].
+  all: try (rewrite Hexpression_Hdeepown_operator Hoperator; wp_auto).
+  all: try lazymatch goal with
+  | Hoperator : LabelSelectorRequirementV.Operator' ?expression = _ |- _ =>
+      destruct expression.(LabelSelectorRequirementV.Values') as [values|]
+        eqn:Hvalues_opt
+  end.
+  all: try lazymatch goal with
+  | Hvalues_opt : LabelSelectorRequirementV.Values' ?expression = Some ?values
+      |- _ =>
+      iRename "Hexpression_Hdeepown_values_some" into "Hsource_values";
+      rewrite /LabelSelectorRequirementV.values_list Hvalues_opt /=
+        in Hvalues_valid Hin_values Hexists_values
+  | Hvalues_opt : LabelSelectorRequirementV.Values' ?expression = None
+      |- _ =>
+      rewrite /LabelSelectorRequirementV.values_list Hvalues_opt /=
+        in Hvalues_valid Hin_values Hexists_values
+  end.
+  1: finish_expression "in"%go values
+    (v1.LabelSelectorRequirement.Values' expression_c) dq Hvalid_expression.
+  1: (exfalso; apply (Hin_values (or_introl Hoperator))).
+  1: done.
+  1: finish_expression "notin"%go values
+    (v1.LabelSelectorRequirement.Values' expression_c) dq Hvalid_expression.
+  1: (exfalso; apply (Hin_values (or_intror Hoperator))).
+  1: done.
+  1: finish_expression "exists"%go values
+    (v1.LabelSelectorRequirement.Values' expression_c) dq Hvalid_expression.
+  1: finish_expression "exists"%go ([] : list go_string) slice.nil dq
+    Hvalid_expression.
+  1: finish_expression "!"%go values
+    (v1.LabelSelectorRequirement.Values' expression_c) dq Hvalid_expression.
+  1: finish_expression "!"%go ([] : list go_string) slice.nil dq
+    Hvalid_expression.
+
+  1: assert (sint.nat loop_i = length expressions) as Hloop_done by word.
+  1: assert (take (sint.nat loop_i) expressions = expressions) as Htake_all.
+  1: { apply take_ge. lia. }
+  1: rewrite Htake_all in Hexpression_entries_pure.
+  1: pose proof (Forall2_length Hexpression_entries_pure)
+    as Hexpression_entries_len.
+  1: rewrite length_fmap in Hexpression_entries_len.
+  1: assert (Forall LabelRequirementV.supported
+      (snd <$> expression_entries)) as Hsupported.
+  1: { eapply expression_conversions_supported.
+       exact Hexpression_entries_pure. }
+  1: assert (Z.of_nat (length expression_entries) ≤ 2 ^ 63 - 1)
+    as Hentries_size.
+  1: { rewrite <- Hexpression_entries_len. simpl in Hsize. lia. }
+  1: iAssert (by_key_contents current_sl expression_entries)
+    with "[Hrequirements Hexpression_entries]"
+    as "Hrequirements_contents".
+  1: { rewrite /by_key_contents.
+       iFrame "Hrequirements". iFrame "#". }
+  1: wp_apply wp_NewSelector.
+  1: iIntros (empty_selector) "[%Hempty_selector #Hempty_selector_rep]".
+  1: rewrite Hempty_selector.
+  1: wp_auto.
+  1: wp_apply (wp_empty_internalSelector__Add current_sl expression_entries
+    with "[$Hlabels_init $Hrequirements_contents]"); first exact Hentries_size.
+  1: exact Hsupported.
+  1: iIntros (converted) "#Hconverted".
+  1: wp_auto.
+  1: iApply "HΦ".
+  1: iSplitR "Hconverted".
+  1: iCombineNamed "Hselector_field_*" as "Hselector_fields".
+  1: iAssert (typed_pointsto_def selector_l selector_c dq)
+    with "[Hselector_fields]" as "Hselector_l".
+  1: { iNamed "Hselector_fields". simpl.
+       rewrite /named Hlabels_map_nil. iFrame. }
+  1: iDestruct (struct_fields_combine (V:=v1.LabelSelector.t)
+    selector_l selector_c dq Hselector_nonnull with "Hselector_l") as
+    "Hselector_l".
+  1: iExists selector_c.
+  1: iFrame "Hselector_l".
+  1: rewrite /LabelSelectorV.deepown /named Hlabels_opt
+    Hexpressions_opt /=.
+  1: iFrame.
+  1: iFrame "%".
+  1: assert (∀ labels_set,
+      selector_matches (snd <$> expression_entries) labels_set ↔
+      LabelSelectorV.matches selector labels_set) as Hmatches.
+  1: { intros labels_set.
+       rewrite (expression_conversions_match expressions
+         (snd <$> expression_entries) labels_set
+         Hexpression_entries_pure).
+       rewrite /LabelSelectorV.matches
+         /LabelSelectorV.match_expressions_list Hlabels_opt
+         Hexpressions_opt /=.
+       split.
+       - intros Hmatch. split; [done|exact Hmatch].
+       - intros [_ Hmatch]. exact Hmatch. }
+  1: iPoseProof (is_selector_ext converted
+    (selector_matches (snd <$> expression_entries))
+    (LabelSelectorV.matches selector) Hmatches with "Hconverted") as
+    "Hconverted'".
+  1: iExact "Hconverted'".
+Qed.
+
+End proof.
