src/proof/k8s_io/apimachinery/pkg/apis/meta/v1_label_selector_conversion.v
@@ -1,0 +1,269 @@
+From New.proof Require Import prelude empty_ffi.
+From New.proof.k8s_io.apimachinery.pkg Require Export labels_add.
+From New.proof.kubernetes_types Require Import labelselector.
+
+Section proof.
+Context `{hG: !heapGS Σ} `{!ffi_semantics _ _}.
+Context {sem : go.Semantics}
+  {labels_sem : labels.Assumptions}
+  {meta_v1_sem : code.k8s_io.apimachinery.pkg.apis.meta.v1.v1.Assumptions}.
+Local Set Default Proof Using "All".
+
+Definition map_label_requirement (key value : go_string) :
+    LabelRequirementV.t :=
+  LabelRequirementV.mk key "="%go [value].
+
+Definition expression_converts
+    (api : LabelSelectorRequirementV.t)
+    (requirement : LabelRequirementV.t) : Prop :=
+  requirement.(LabelRequirementV.Key') =
+      api.(LabelSelectorRequirementV.Key') ∧
+  requirement.(LabelRequirementV.Values') =
+      LabelSelectorRequirementV.values_list api ∧
+  ((api.(LabelSelectorRequirementV.Operator') = "In"%go ∧
+      requirement.(LabelRequirementV.Operator') = "in"%go) ∨
+    (api.(LabelSelectorRequirementV.Operator') = "NotIn"%go ∧
+      requirement.(LabelRequirementV.Operator') = "notin"%go) ∨
+    (api.(LabelSelectorRequirementV.Operator') = "Exists"%go ∧
+      requirement.(LabelRequirementV.Operator') = "exists"%go) ∨
+    (api.(LabelSelectorRequirementV.Operator') = "DoesNotExist"%go ∧
+      requirement.(LabelRequirementV.Operator') = "!"%go)).
+
+Lemma expression_converts_supported api requirement :
+  expression_converts api requirement →
+  LabelRequirementV.supported requirement.
+Proof.
+  intros (_ & _ & Hop).
+  destruct Hop as [[_ Hrequirement]|[[_ Hrequirement]|
+      [[_ Hrequirement]|[_ Hrequirement]]]];
+    rewrite /LabelRequirementV.supported Hrequirement /=; tauto.
+Qed.
+
+Lemma valid_expression_conversion api :
+  LabelSelectorRequirementV.valid api →
+  ∃ requirement,
+    expression_converts api requirement ∧
+    valid_requirement_inputs
+      requirement.(LabelRequirementV.Key')
+      requirement.(LabelRequirementV.Operator')
+      requirement.(LabelRequirementV.Values').
+Proof.
+  intros (Hop & Hin & Hexists & Hkey & Hvalues).
+  destruct Hop as [Hop|[Hop|[Hop|Hop]]].
+  - exists (LabelRequirementV.mk api.(LabelSelectorRequirementV.Key')
+      "in"%go (LabelSelectorRequirementV.values_list api)).
+    split; [rewrite /expression_converts /=; tauto|].
+    rewrite /valid_requirement_inputs /=. split_and!; try done.
+    left. split; [left; done|]. apply Hin. tauto.
+  - exists (LabelRequirementV.mk api.(LabelSelectorRequirementV.Key')
+      "notin"%go (LabelSelectorRequirementV.values_list api)).
+    split; [rewrite /expression_converts /=; tauto|].
+    rewrite /valid_requirement_inputs /=. split_and!; try done.
+    left. split; [right; done|]. apply Hin. tauto.
+  - exists (LabelRequirementV.mk api.(LabelSelectorRequirementV.Key')
+      "exists"%go (LabelSelectorRequirementV.values_list api)).
+    split; [rewrite /expression_converts /=; tauto|].
+    rewrite /valid_requirement_inputs /=. split_and!; try done.
+    right. right. split; [left; done|]. apply Hexists. tauto.
+  - exists (LabelRequirementV.mk api.(LabelSelectorRequirementV.Key')
+      "!"%go (LabelSelectorRequirementV.values_list api)).
+    split; [rewrite /expression_converts /=; tauto|].
+    rewrite /valid_requirement_inputs /=. split_and!; try done.
+    right. right. split; [right; done|]. apply Hexists. tauto.
+Qed.
+
+Lemma expression_converts_valid_inputs api requirement :
+  LabelSelectorRequirementV.valid api →
+  expression_converts api requirement →
+  valid_requirement_inputs
+    requirement.(LabelRequirementV.Key')
+    requirement.(LabelRequirementV.Operator')
+    requirement.(LabelRequirementV.Values').
+Proof.
+  intros (Hop_valid & Hin & Hexists & Hkey_valid & Hvalues_valid)
+    (Hkey & Hvalues & Hop).
+  rewrite /valid_requirement_inputs Hkey Hvalues.
+  split_and!; try done.
+  destruct Hop as [[Hapi Hop]|[[Hapi Hop]|[[Hapi Hop]|[Hapi Hop]]]].
+  - rewrite Hop. left. split; [left; done|]. apply Hin. tauto.
+  - rewrite Hop. left. split; [right; done|]. apply Hin. tauto.
+  - rewrite Hop. right. right. split; [left; done|].
+    apply Hexists. tauto.
+  - rewrite Hop. right. right. split; [right; done|].
+    apply Hexists. tauto.
+Qed.
+
+Lemma expression_converts_matches api requirement labels_set :
+  expression_converts api requirement →
+  LabelRequirementV.matches requirement labels_set ↔
+    LabelSelectorV.requirement_matches labels_set api.
+Proof.
+  intros (Hkey & Hvalues & Hop).
+  destruct Hop as [[Hapi Hop]|[[Hapi Hop]|[[Hapi Hop]|[Hapi Hop]]]].
+  all: rewrite /LabelRequirementV.matches
+      /LabelSelectorV.requirement_matches
+      /LabelRequirementV.selected_label /LabelSelectorV.selected_label
+      Hkey Hvalues Hapi Hop /=.
+  all: destruct labels_set as [label_map|]; simpl.
+  all: try destruct (label_map !! api.(LabelSelectorRequirementV.Key'));
+    simpl.
+  Timeout 10 all: set_solver.
+Qed.
+
+Lemma map_label_requirement_matches key value labels_set :
+  LabelRequirementV.matches (map_label_requirement key value) labels_set ↔
+  LabelSelectorV.selected_label labels_set key = Some value.
+Proof.
+  rewrite /map_label_requirement /LabelRequirementV.matches
+    /LabelRequirementV.selected_label /LabelSelectorV.selected_label /=.
+  destruct labels_set as [labels_set|]; simpl.
+  all: try destruct (labels_set !! key); simpl.
+  Timeout 10 all: set_solver.
+Qed.
+
+Lemma selector_matches_snoc requirements requirement labels_set :
+  selector_matches (requirements ++ [requirement]) labels_set ↔
+  selector_matches requirements labels_set ∧
+    LabelRequirementV.matches requirement labels_set.
+Proof. rewrite /selector_matches Forall_app Forall_singleton. done. Qed.
+
+Fixpoint map_requirements (keys : list go_string)
+    (labels_map : gmap go_string go_string) : list LabelRequirementV.t :=
+  match keys with
+  | [] => []
+  | key :: keys =>
+      match labels_map !! key with
+      | Some value =>
+          map_label_requirement key value :: map_requirements keys labels_map
+      | None => map_requirements keys labels_map
+      end
+  end.
+
+Lemma elem_of_map_requirements requirement keys labels_map :
+  requirement ∈ map_requirements keys labels_map ↔
+  ∃ key value, key ∈ keys ∧ labels_map !! key = Some value ∧
+    requirement = map_label_requirement key value.
+Proof.
+  induction keys as [|key keys IH]; simpl.
+  { Timeout 10 set_solver. }
+  destruct (labels_map !! key) as [value|] eqn:Hlookup; simpl.
+  - rewrite elem_of_cons IH. Timeout 10 set_solver.
+  - rewrite IH. Timeout 10 set_solver.
+Qed.
+
+Lemma map_requirements_snoc keys labels_map key value :
+  labels_map !! key = Some value →
+  map_requirements (keys ++ [key]) labels_map =
+    map_requirements keys labels_map ++ [map_label_requirement key value].
+Proof.
+  intros Hlookup. induction keys as [|head keys IH]; simpl.
+  - rewrite Hlookup. done.
+  - destruct (labels_map !! head); simpl; rewrite IH; done.
+Qed.
+
+Lemma map_requirements_length keys labels_map :
+  (∀ key, In key keys → ∃ value, labels_map !! key = Some value) →
+  length (map_requirements keys labels_map) = length keys.
+Proof.
+  intros Hlookup. induction keys as [|key keys IH]; simpl; first done.
+  destruct (Hlookup key (or_introl eq_refl)) as [value Hvalue].
+  rewrite Hvalue /=. f_equal. apply IH.
+  intros key' Hkey'. apply Hlookup. right. exact Hkey'.
+Qed.
+
+Lemma map_requirements_supported keys labels_map :
+  Forall LabelRequirementV.supported (map_requirements keys labels_map).
+Proof.
+  induction keys as [|key keys IH]; simpl; first constructor.
+  destruct (labels_map !! key) as [value|]; last exact IH.
+  constructor; last exact IH.
+  rewrite /map_label_requirement /LabelRequirementV.supported /=. tauto.
+Qed.
+
+Lemma expression_conversions_supported apis requirements :
+  Forall2 expression_converts apis requirements →
+  Forall LabelRequirementV.supported requirements.
+Proof.
+  intros Hconverts. induction Hconverts as
+    [|api requirement apis requirements Hconvert _ IH].
+  - constructor.
+  - constructor.
+    + eapply expression_converts_supported. exact Hconvert.
+    + exact IH.
+Qed.
+
+Lemma Forall2_nil_left {A B} (R : A → B → Prop) ys :
+  Forall2 R [] ys → ys = [].
+Proof. intros Hrelated. inversion Hrelated. done. Qed.
+
+Lemma fmap_eq_nil {A B} (f : A → B) xs :
+  f <$> xs = [] → xs = [].
+Proof. destruct xs; simpl; [done|discriminate]. Qed.
+
+Lemma map_requirements_match keys labels_map labels_set :
+  list_to_set keys = dom labels_map →
+  selector_matches (map_requirements keys labels_map) labels_set ↔
+    LabelSelectorV.match_labels (Some labels_map) labels_set.
+Proof.
+  intros Hdom. rewrite /selector_matches.
+  destruct labels_set as [labels_set|].
+  - rewrite /LabelSelectorV.match_labels Forall_forall.
+    split; intros Hmatch.
+    + intros key value Hlookup.
+      apply (proj1 (map_label_requirement_matches key value (Some labels_set))).
+      apply Hmatch. rewrite <-list_elem_of_In.
+      apply (proj2 (elem_of_map_requirements _ _ _)).
+      exists key, value. repeat split; try done.
+      rewrite <-(elem_of_list_to_set (C:=gset go_string)).
+      rewrite Hdom elem_of_dom. eauto.
+    + intros requirement Hin.
+      rewrite <-list_elem_of_In in Hin.
+      apply (proj1 (elem_of_map_requirements _ _ _)) in Hin as
+        (key & value & _ & Hlookup & ->).
+      apply (proj2 (map_label_requirement_matches key value (Some labels_set))).
+      apply Hmatch. exact Hlookup.
+  - rewrite /LabelSelectorV.match_labels Forall_forall.
+    split; intros Hmatch.
+    + apply map_eq. intros key.
+      rewrite lookup_empty.
+      destruct (labels_map !! key) as [value|] eqn:Hlookup; last done.
+      exfalso.
+      specialize (Hmatch (map_label_requirement key value)).
+      rewrite map_label_requirement_matches in Hmatch.
+      assert (In (map_label_requirement key value)
+        (map_requirements keys labels_map)) as Hin.
+      { rewrite <-list_elem_of_In.
+        apply (proj2 (elem_of_map_requirements _ _ _)).
+        exists key, value. repeat split; try done.
+        rewrite <-(elem_of_list_to_set (C:=gset go_string)).
+        rewrite Hdom elem_of_dom. eauto. }
+      specialize (Hmatch Hin).
+      rewrite /LabelSelectorV.selected_label in Hmatch. discriminate.
+    + subst labels_map.
+      assert (keys = []) as ->.
+      { destruct keys as [|key keys]; first done.
+        exfalso. assert (key ∈
+          list_to_set (C:=gset go_string) (key :: keys)) as Hkey.
+        { Timeout 10 set_solver. }
+        rewrite Hdom dom_empty elem_of_empty in Hkey. done. }
+      intros requirement Hfalse. inversion Hfalse.
+Qed.
+
+Lemma expression_conversions_match apis requirements labels_set :
+  Forall2 expression_converts apis requirements →
+  selector_matches requirements labels_set ↔
+    Forall (LabelSelectorV.requirement_matches labels_set) apis.
+Proof.
+  intros Hrelated. rewrite /selector_matches.
+  induction Hrelated as [|api requirement apis requirements Hconvert _ IH];
+    simpl; first done.
+  split; intros Hall.
+  - inversion Hall as [|? ? Hhead Htail]. constructor.
+    + apply (proj1 (expression_converts_matches _ _ _ Hconvert)). exact Hhead.
+    + apply (proj1 IH). exact Htail.
+  - inversion Hall as [|? ? Hhead Htail]. constructor.
+    + apply (proj2 (expression_converts_matches _ _ _ Hconvert)). exact Hhead.
+    + apply (proj2 IH). exact Htail.
+Qed.
+
+End proof.
