src/proof/k8s_io/apimachinery/pkg/labels.v
@@ -1,0 +1,682 @@
+From New.proof Require Import prelude empty_ffi.
+From New.proof.k8s_io.apimachinery.pkg Require Export labels_init.
+
+Module LabelRequirementV.
+
+Record t := mk {
+  Key' : go_string;
+  Operator' : selection.Operator.t;
+  Values' : list go_string;
+}.
+
+Global Instance eq_dec : EqDecision t.
+Proof. solve_decision. Defined.
+
+Definition selected_label
+    (ls : option (gmap go_string go_string)) (key : go_string) :
+    option go_string :=
+  match ls with
+  | Some labels => labels !! key
+  | None => None
+  end.
+
+Definition matches
+    (r : t) (ls : option (gmap go_string go_string)) : Prop :=
+  ((r.(Operator') = "in"%go ∨ r.(Operator') = "="%go ∨
+      r.(Operator') = "=="%go) ∧
+    match selected_label ls r.(Key') with
+    | Some value => value ∈ r.(Values')
+    | None => False
+    end) ∨
+  ((r.(Operator') = "notin"%go ∨ r.(Operator') = "!="%go) ∧
+    match selected_label ls r.(Key') with
+    | Some value => value ∉ r.(Values')
+    | None => True
+    end) ∨
+  (r.(Operator') = "exists"%go ∧ is_Some (selected_label ls r.(Key'))) ∨
+  (r.(Operator') = "!"%go ∧ selected_label ls r.(Key') = None).
+
+Definition supported (r : t) : Prop :=
+  r.(Operator') = "in"%go ∨ r.(Operator') = "="%go ∨
+  r.(Operator') = "=="%go ∨ r.(Operator') = "notin"%go ∨
+  r.(Operator') = "!="%go ∨ r.(Operator') = "exists"%go ∨
+  r.(Operator') = "!"%go.
+
+Global Instance matches_dec r ls : Decision (matches r ls).
+Proof. unfold matches. destruct (selected_label ls r.(Key')); apply _. Defined.
+
+End LabelRequirementV.
+
+Section proof.
+Context `{hG: !heapGS Σ} `{!ffi_semantics _ _}.
+Context {sem : go.Semantics} {package_sem : labels.Assumptions}.
+Collection W := sem + package_sem.
+Local Set Default Proof Using "All".
+
+Definition labels_set_rep (l : map.t)
+    (ls : option (gmap go_string go_string)) (dq : dfrac) : iProp Σ :=
+  ⌜ l = null ↔ ls = None ⌝ ∗
+  match ls with
+  | Some m => l ↦${dq} m
+  | None => True
+  end.
+
+Global Instance labels_set_rep_persistent l ls :
+  Persistent (labels_set_rep l ls DfracDiscarded).
+Proof. rewrite /labels_set_rep. apply _. Qed.
+
+Definition label_requirement_rep (c : labels.Requirement.t)
+    (r : LabelRequirementV.t) : iProp Σ :=
+  ⌜ c.(labels.Requirement.key') = r.(LabelRequirementV.Key') ⌝ ∗
+  ⌜ c.(labels.Requirement.operator') = r.(LabelRequirementV.Operator') ⌝ ∗
+  c.(labels.Requirement.strValues') ↦*□ r.(LabelRequirementV.Values').
+
+Global Instance label_requirement_rep_persistent c r :
+  Persistent (label_requirement_rep c r).
+Proof. rewrite /label_requirement_rep. apply _. Qed.
+
+Definition selector_matches
+    (requirements : list LabelRequirementV.t)
+    (ls : option (gmap go_string go_string)) : Prop :=
+  Forall (λ requirement, LabelRequirementV.matches requirement ls) requirements.
+
+Global Instance selector_matches_dec requirements ls :
+  Decision (selector_matches requirements ls).
+Proof. unfold selector_matches. apply _. Defined.
+
+Definition everything_matches (_ : option (gmap go_string go_string)) : Prop := True.
+Definition nothing_matches (_ : option (gmap go_string go_string)) : Prop := False.
+
+Global Instance everything_matches_dec ls : Decision (everything_matches ls).
+Proof. unfold everything_matches. apply _. Defined.
+
+Global Instance nothing_matches_dec ls : Decision (nothing_matches ls).
+Proof. unfold nothing_matches. apply _. Defined.
+
+Definition is_selector (selector : labels.Selector.t)
+    (P : option (gmap go_string go_string) → Prop) : iProp Σ :=
+  (∃ sl cs requirements,
+    ⌜ selector = interface.ok (interface.mk labels.internalSelector #sl) ⌝ ∗
+    sl ↦*□ cs ∗
+    ([∗ list] c;r ∈ cs;requirements, label_requirement_rep c r) ∗
+    ⌜ Forall LabelRequirementV.supported requirements ⌝ ∗
+    ⌜ ∀ ls, P ls ↔ selector_matches requirements ls ⌝) ∨
+  (⌜ selector = interface.ok (interface.mk labels.nothingSelector #(labels.nothingSelector.mk)) ⌝ ∗
+    ⌜ ∀ ls, ¬ P ls ⌝).
+
+Global Instance is_selector_persistent selector P :
+  Persistent (is_selector selector P).
+Proof. rewrite /is_selector. apply _. Qed.
+
+Lemma wp_Set__Has l ls dq key :
+  {{{ labels_set_rep l ls dq }}}
+    l @! labels.Set' @! "Has" #key
+  {{{ b, RET #b;
+      labels_set_rep l ls dq ∗
+      ⌜ b = bool_decide (is_Some (LabelRequirementV.selected_label ls key)) ⌝
+  }}}.
+Proof.
+  wp_start as "H".
+  rewrite /labels_set_rep.
+  iDestruct "H" as "[%Hl Hmap]".
+  wp_auto.
+  destruct ls as [m|].
+  - wp_apply (wp_map_lookup2 with "Hmap") as "Hmap".
+    iApply "HΦ". iSplit.
+    { iSplit.
+      - iPureIntro. exact Hl.
+      - iExact "Hmap". }
+    iPureIntro. destruct (m !! key) as [value|] eqn:Hlookup;
+      rewrite /LabelRequirementV.selected_label Hlookup; simpl; done.
+  - assert (l = null) as -> by (apply Hl; done). wp_auto.
+    iApply "HΦ". iSplit; [iSplit; done|done].
+Qed.
+
+Lemma wp_Set__Lookup l ls dq key :
+  {{{ labels_set_rep l ls dq }}}
+    l @! labels.Set' @! "Lookup" #key
+  {{{ value b, RET (#value, #b);
+      labels_set_rep l ls dq ∗
+      ⌜ (b = true ∧ LabelRequirementV.selected_label ls key = Some value) ∨
+        (b = false ∧ LabelRequirementV.selected_label ls key = None) ⌝
+  }}}.
+Proof.
+  wp_start as "H".
+  rewrite /labels_set_rep.
+  iDestruct "H" as "[%Hl Hmap]".
+  wp_auto.
+  destruct ls as [m|].
+  - wp_apply (wp_map_lookup2 with "Hmap") as "Hmap".
+    iApply "HΦ". iSplit.
+    { iSplit.
+      - iPureIntro. exact Hl.
+      - iExact "Hmap". }
+    iPureIntro. destruct (m !! key) as [value|] eqn:Hlookup;
+      rewrite /LabelRequirementV.selected_label Hlookup; simpl; eauto.
+  - assert (l = null) as -> by (apply Hl; done). wp_auto.
+    iApply "HΦ". iSplit; [iSplit; done|eauto].
+Qed.
+
+Lemma wp_Requirement__hasValue r_l c r dq value :
+  {{{ r_l ↦{dq} c ∗ label_requirement_rep c r }}}
+    r_l @! (go.PointerType labels.Requirement) @! "hasValue" #value
+  {{{ b, RET #b;
+      r_l ↦{dq} c ∗
+      label_requirement_rep c r ∗
+      ⌜ b = bool_decide (value ∈ r.(LabelRequirementV.Values')) ⌝
+  }}}.
+Proof.
+  wp_start as "H". iDestruct "H" as "[Hr #Hrep]".
+  rewrite /label_requirement_rep.
+  iDestruct "Hrep" as "(%Hkey & %Hop & #Hvalues)".
+  rewrite exception_do_unseal /exception_do_def.
+  wp_auto.
+  iDestruct (own_slice_len with "Hvalues") as %[Hlen Hlen_nonneg].
+  wp_alloc loop_i_ptr as "Hloop_i". wp_auto.
+  set I := (∃ (loop_i source_i : w64),
+    "Hloop_i" ∷ loop_i_ptr ↦ loop_i ∗
+    "Hi" ∷ i_ptr ↦ source_i ∗
+    "Hr" ∷ r_l ↦{dq} c ∗
+    "%Hi_bounds" ∷ ⌜ 0 ≤ sint.Z loop_i ≤ length r.(LabelRequirementV.Values') ⌝ ∗
+    "%Hnot_found" ∷ ⌜ value ∉ take (sint.nat loop_i) r.(LabelRequirementV.Values') ⌝)%I.
+  iAssert I with "[Hloop_i i Hr]" as "Hloop".
+  { iExists (W64 0), (W64 0). iFrame. iPureIntro. split; first word.
+    simpl. intros Hmember. inversion Hmember. }
+  wp_for "Hloop". wp_if_destruct.
+  - assert (0 ≤ sint.Z loop_i < length r.(LabelRequirementV.Values')) as Hibounds by word.
+    assert (0 ≤ sint.Z loop_i < sint.Z (slice.len c.(labels.Requirement.strValues')))
+      as Hslice_bounds by word.
+    list_elem r.(LabelRequirementV.Values') (sint.Z loop_i) as current.
+    rewrite decide_True; [exact Hslice_bounds|].
+    wp_apply (wp_load_slice_index with "[$Hvalues]");
+      [word|iPureIntro; exact Hcurrent_lookup|].
+    iIntros "_". wp_auto.
+    rewrite decide_True; [exact Hslice_bounds|].
+    wp_apply (wp_load_slice_index with "[$Hvalues]");
+      [word|iPureIntro; exact Hcurrent_lookup|].
+    iIntros "_". wp_auto. wp_if_destruct.
+    + iApply wp_for_post_return.
+      rewrite return_val_unseal /return_val_def. wp_auto.
+      rewrite exception_seq_unseal /exception.exception_seq_def. wp_auto.
+      iApply "HΦ". iFrame. iFrame "#". iPureIntro.
+      assert (value ∈ r.(LabelRequirementV.Values')) as Hmember.
+      { eapply list_elem_of_lookup_2. exact Hcurrent_lookup. }
+      rewrite bool_decide_true; done.
+    + iApply wp_for_post_do. wp_auto.
+      iFrame "HΦ r value".
+      iExists (word.add loop_i (W64 1)), loop_i. iFrame.
+      iPureIntro. split; first word.
+      assert (sint.nat (word.add loop_i (W64 1)) = S (sint.nat loop_i)) as -> by word.
+      rewrite (take_S_r _ _ current Hcurrent_lookup).
+      apply not_elem_of_app. split; first done.
+      rewrite list_elem_of_singleton. intros Heq.
+      apply n. symmetry. exact Heq.
+  - assert (sint.nat loop_i = length r.(LabelRequirementV.Values')) as Hi_len by word.
+    assert (take (sint.nat loop_i) r.(LabelRequirementV.Values') =
+      r.(LabelRequirementV.Values')) as Htake.
+    { apply take_ge. rewrite Hi_len. done. }
+    rewrite Htake in Hnot_found.
+    rewrite return_val_unseal /return_val_def. wp_auto.
+    iApply "HΦ". iFrame. iFrame "#". iPureIntro.
+    rewrite bool_decide_false; done.
+Qed.
+
+Lemma wp_Requirement__Matches_impl r_l c r dq labels_l ls labels_dq :
+  LabelRequirementV.supported r →
+  {{{ r_l ↦{dq} c ∗
+      label_requirement_rep c r ∗
+      labels_set_rep labels_l ls labels_dq
+  }}}
+    (labels.Requirement__Matchesⁱᵐᵖˡ #r_l)
+      #(interface.ok (interface.mk labels.Set' #labels_l))
+  {{{ b, RET #b;
+      r_l ↦{dq} c ∗
+      label_requirement_rep c r ∗
+      labels_set_rep labels_l ls labels_dq ∗
+      ⌜ b = bool_decide (LabelRequirementV.matches r ls) ⌝
+  }}}.
+Proof.
+  intros Hsupported.
+  wp_start as "H".
+  iDestruct "H" as "(r_l & label_requirement_rep & labels_set_rep)".
+  iEval (rewrite /label_requirement_rep) in "label_requirement_rep".
+  iDestruct "label_requirement_rep" as "(%Hkey & %Hop & #Hvalues)".
+  iAssert (label_requirement_rep c r) as "#Hrep".
+  { rewrite /label_requirement_rep. iFrame "#%". }
+  rewrite exception_do_unseal /exception_do_def.
+  wp_auto.
+  destruct Hsupported as [Hin|[Heq|[Hdeq|[Hnotin|[Hneq|[Hexists|Hnotexists]]]]]];
+    rewrite Hop; rewrite ?Hin ?Heq ?Hdeq ?Hnotin ?Hneq ?Hexists ?Hnotexists;
+    wp_auto; rewrite Hkey.
+  - wp_apply (wp_Set__Lookup with "[$labels_set_rep]").
+    iIntros (found_value found) "[Hlabels %Hfound]".
+    destruct Hfound as [[-> Hfound]|[-> Hfound]].
+    + wp_auto.
+      wp_apply (wp_Requirement__hasValue with "[$r_l $Hvalues //]").
+      iIntros (b) "(Hr & _ & %Hb)".
+      wp_auto. rewrite return_val_unseal /return_val_def. wp_auto.
+      iApply "HΦ". iFrame. iFrame "#". iPureIntro.
+      rewrite Hb. apply bool_decide_ext.
+      unfold LabelRequirementV.matches. rewrite Hin Hfound.
+      split.
+      * intros Hmember. left. split; [left; reflexivity|exact Hmember].
+      * intros [Hgood|[Hnot|[Hexists'|Hdoesnot]]].
+        { destruct Hgood as [_ Hmember]. exact Hmember. }
+        { destruct Hnot as [[Hbad|Hbad] _]; discriminate. }
+        { destruct Hexists' as [Hbad _]. discriminate. }
+        { destruct Hdoesnot as [Hbad _]. discriminate. }
+    + wp_auto. rewrite return_val_unseal /return_val_def. wp_auto.
+      iApply "HΦ". iFrame. iFrame "#". iPureIntro.
+      symmetry. apply bool_decide_eq_false_2.
+      unfold LabelRequirementV.matches. rewrite Hin Hfound.
+      intros [Hgood|[Hnot|[Hexists'|Hdoesnot]]].
+      * destruct Hgood as [_ Hfalse]. exact Hfalse.
+      * destruct Hnot as [[Hbad|Hbad] _]; discriminate.
+      * destruct Hexists' as [Hbad _]. discriminate.
+      * destruct Hdoesnot as [Hbad _]. discriminate.
+  - wp_apply (wp_Set__Lookup with "[$labels_set_rep]").
+    iIntros (found_value found) "[Hlabels %Hfound]".
+    destruct Hfound as [[-> Hfound]|[-> Hfound]].
+    + wp_auto.
+      wp_apply (wp_Requirement__hasValue with "[$r_l $Hvalues //]").
+      iIntros (b) "(Hr & _ & %Hb)".
+      wp_auto. rewrite return_val_unseal /return_val_def. wp_auto.
+      iApply "HΦ". iFrame. iFrame "#". iPureIntro.
+      rewrite Hb. apply bool_decide_ext.
+      unfold LabelRequirementV.matches. rewrite Heq Hfound.
+      split.
+      * intros Hmember. left. split; [right; left; reflexivity|exact Hmember].
+      * intros [Hgood|[Hnot|[Hexists'|Hdoesnot]]].
+        { destruct Hgood as [_ Hmember]. exact Hmember. }
+        { destruct Hnot as [[Hbad|Hbad] _]; discriminate. }
+        { destruct Hexists' as [Hbad _]. discriminate. }
+        { destruct Hdoesnot as [Hbad _]. discriminate. }
+    + wp_auto. rewrite return_val_unseal /return_val_def. wp_auto.
+      iApply "HΦ". iFrame. iFrame "#". iPureIntro.
+      symmetry. apply bool_decide_eq_false_2.
+      unfold LabelRequirementV.matches. rewrite Heq Hfound.
+      intros [Hgood|[Hnot|[Hexists'|Hdoesnot]]].
+      * destruct Hgood as [_ Hfalse]. exact Hfalse.
+      * destruct Hnot as [[Hbad|Hbad] _]; discriminate.
+      * destruct Hexists' as [Hbad _]. discriminate.
+      * destruct Hdoesnot as [Hbad _]. discriminate.
+  - wp_apply (wp_Set__Lookup with "[$labels_set_rep]").
+    iIntros (found_value found) "[Hlabels %Hfound]".
+    destruct Hfound as [[-> Hfound]|[-> Hfound]].
+    + wp_auto.
+      wp_apply (wp_Requirement__hasValue with "[$r_l $Hvalues //]").
+      iIntros (b) "(Hr & _ & %Hb)".
+      wp_auto. rewrite return_val_unseal /return_val_def. wp_auto.
+      iApply "HΦ". iFrame. iFrame "#". iPureIntro.
+      rewrite Hb. apply bool_decide_ext.
+      unfold LabelRequirementV.matches. rewrite Hdeq Hfound.
+      split.
+      * intros Hmember. left. split; [right; right; reflexivity|exact Hmember].
+      * intros [Hgood|[Hnot|[Hexists'|Hdoesnot]]].
+        { destruct Hgood as [_ Hmember]. exact Hmember. }
+        { destruct Hnot as [[Hbad|Hbad] _]; discriminate. }
+        { destruct Hexists' as [Hbad _]. discriminate. }
+        { destruct Hdoesnot as [Hbad _]. discriminate. }
+    + wp_auto. rewrite return_val_unseal /return_val_def. wp_auto.
+      iApply "HΦ". iFrame. iFrame "#". iPureIntro.
+      symmetry. apply bool_decide_eq_false_2.
+      unfold LabelRequirementV.matches. rewrite Hdeq Hfound.
+      intros [Hgood|[Hnot|[Hexists'|Hdoesnot]]].
+      * destruct Hgood as [_ Hfalse]. exact Hfalse.
+      * destruct Hnot as [[Hbad|Hbad] _]; discriminate.
+      * destruct Hexists' as [Hbad _]. discriminate.
+      * destruct Hdoesnot as [Hbad _]. discriminate.
+  - wp_apply (wp_Set__Lookup with "[$labels_set_rep]").
+    iIntros (found_value found) "[Hlabels %Hfound]".
+    destruct Hfound as [[-> Hfound]|[-> Hfound]].
+    + wp_auto.
+      wp_apply (wp_Requirement__hasValue with "[$r_l $Hvalues //]").
+      iIntros (b) "(Hr & _ & %Hb)".
+      wp_auto. rewrite return_val_unseal /return_val_def. wp_auto.
+      iApply "HΦ". iFrame. iFrame "#". iPureIntro.
+      destruct (decide (found_value ∈ r.(LabelRequirementV.Values'))) as [Hmem|Hmem].
+      * assert (bool_decide (found_value ∈ r.(LabelRequirementV.Values')) = true)
+          as Hbool by (apply bool_decide_eq_true_2; exact Hmem).
+        rewrite Hb Hbool. simpl.
+        symmetry. apply bool_decide_eq_false_2.
+        unfold LabelRequirementV.matches. rewrite Hnotin Hfound.
+        intros [Hfirst|[Hsecond|[Hexists'|Hdoesnot]]].
+        { destruct Hfirst as [[Hbad|[Hbad|Hbad]] _]; discriminate. }
+        { destruct Hsecond as [_ Hnotmember]. exact (Hnotmember Hmem). }
+        { destruct Hexists' as [Hbad _]. discriminate. }
+        { destruct Hdoesnot as [Hbad _]. discriminate. }
+      * assert (bool_decide (found_value ∈ r.(LabelRequirementV.Values')) = false)
+          as Hbool by (apply bool_decide_eq_false_2; exact Hmem).
+        rewrite Hb Hbool. simpl.
+        symmetry. apply bool_decide_eq_true_2.
+        unfold LabelRequirementV.matches. rewrite Hnotin Hfound.
+        right. left. split; [left; reflexivity|exact Hmem].
+    + wp_auto. rewrite return_val_unseal /return_val_def. wp_auto.
+      iApply "HΦ". iFrame. iFrame "#". iPureIntro.
+      symmetry. apply bool_decide_eq_true_2.
+      unfold LabelRequirementV.matches. rewrite Hnotin Hfound.
+      right. left. split; [left; reflexivity|done].
+  - wp_apply (wp_Set__Lookup with "[$labels_set_rep]").
+    iIntros (found_value found) "[Hlabels %Hfound]".
+    destruct Hfound as [[-> Hfound]|[-> Hfound]].
+    + wp_auto.
+      wp_apply (wp_Requirement__hasValue with "[$r_l $Hvalues //]").
+      iIntros (b) "(Hr & _ & %Hb)".
+      wp_auto. rewrite return_val_unseal /return_val_def. wp_auto.
+      iApply "HΦ". iFrame. iFrame "#". iPureIntro.
+      destruct (decide (found_value ∈ r.(LabelRequirementV.Values'))) as [Hmem|Hmem].
+      * assert (bool_decide (found_value ∈ r.(LabelRequirementV.Values')) = true)
+          as Hbool by (apply bool_decide_eq_true_2; exact Hmem).
+        rewrite Hb Hbool. simpl.
+        symmetry. apply bool_decide_eq_false_2.
+        unfold LabelRequirementV.matches. rewrite Hneq Hfound.
+        intros [Hfirst|[Hsecond|[Hexists'|Hdoesnot]]].
+        { destruct Hfirst as [[Hbad|[Hbad|Hbad]] _]; discriminate. }
+        { destruct Hsecond as [_ Hnotmember]. exact (Hnotmember Hmem). }
+        { destruct Hexists' as [Hbad _]. discriminate. }
+        { destruct Hdoesnot as [Hbad _]. discriminate. }
+      * assert (bool_decide (found_value ∈ r.(LabelRequirementV.Values')) = false)
+          as Hbool by (apply bool_decide_eq_false_2; exact Hmem).
+        rewrite Hb Hbool. simpl.
+        symmetry. apply bool_decide_eq_true_2.
+        unfold LabelRequirementV.matches. rewrite Hneq Hfound.
+        right. left. split; [right; reflexivity|exact Hmem].
+    + wp_auto. rewrite return_val_unseal /return_val_def. wp_auto.
+      iApply "HΦ". iFrame. iFrame "#". iPureIntro.
+      symmetry. apply bool_decide_eq_true_2.
+      unfold LabelRequirementV.matches. rewrite Hneq Hfound.
+      right. left. split; [right; reflexivity|done].
+  - wp_apply (wp_Set__Has with "[$labels_set_rep]").
+    iIntros (b) "[Hlabels %Hb]".
+    wp_auto. rewrite return_val_unseal /return_val_def. wp_auto.
+    iApply "HΦ". iFrame. iFrame "#". iPureIntro.
+    rewrite Hb. apply bool_decide_ext.
+    unfold LabelRequirementV.matches. rewrite Hexists.
+    split.
+    + intros Hsome. right. right. left. split; [reflexivity|exact Hsome].
+    + intros [Hfirst|[Hsecond|[Hexists'|Hdoesnot]]].
+      * destruct Hfirst as [[Hbad|[Hbad|Hbad]] _]; discriminate.
+      * destruct Hsecond as [[Hbad|Hbad] _]; discriminate.
+      * destruct Hexists' as [_ Hsome]. exact Hsome.
+      * destruct Hdoesnot as [Hbad _]. discriminate.
+  - wp_apply (wp_Set__Has with "[$labels_set_rep]").
+    iIntros (b) "[Hlabels %Hb]".
+    wp_auto. rewrite return_val_unseal /return_val_def. wp_auto.
+    iApply "HΦ". iFrame. iFrame "#". iPureIntro.
+    destruct (LabelRequirementV.selected_label ls r.(LabelRequirementV.Key'))
+      as [value'|] eqn:Hselected.
+    + assert (bool_decide (is_Some (Some value')) = true) as Hsome by done.
+      rewrite Hb Hsome. simpl.
+      symmetry. apply bool_decide_eq_false_2.
+      unfold LabelRequirementV.matches. rewrite Hnotexists.
+      intros [Hfirst|[Hsecond|[Hexists'|Hdoesnot]]].
+      * destruct Hfirst as [[Hbad|[Hbad|Hbad]] _]; discriminate.
+      * destruct Hsecond as [[Hbad|Hbad] _]; discriminate.
+      * destruct Hexists' as [Hbad _]. discriminate.
+      * destruct Hdoesnot as [_ Hnone]. rewrite Hselected in Hnone. discriminate.
+    + assert (bool_decide (is_Some (None : option go_string)) = false) as Hnone by done.
+      rewrite Hb Hnone. simpl.
+      symmetry. apply bool_decide_eq_true_2.
+      unfold LabelRequirementV.matches. rewrite Hnotexists.
+      right. right. right. split; [reflexivity|exact Hselected].
+Qed.
+
+Lemma wp_Requirement__Matches r_l c r dq labels_l ls labels_dq :
+  LabelRequirementV.supported r →
+  {{{ r_l ↦{dq} c ∗
+      label_requirement_rep c r ∗
+      labels_set_rep labels_l ls labels_dq
+  }}}
+    r_l @! (go.PointerType labels.Requirement) @! "Matches"
+      #(interface.ok (interface.mk labels.Set' #labels_l))
+  {{{ b, RET #b;
+      r_l ↦{dq} c ∗
+      label_requirement_rep c r ∗
+      labels_set_rep labels_l ls labels_dq ∗
+      ⌜ b = bool_decide (LabelRequirementV.matches r ls) ⌝
+  }}}.
+Proof.
+  intros Hsupported.
+  iIntros (Φ) "H HΦ".
+  wp_method_call. wp_call.
+  wp_apply (wp_Requirement__Matches_impl r_l c r dq labels_l ls labels_dq
+    Hsupported with "H").
+  iIntros (b) "H". iApply "HΦ". iExact "H".
+Qed.
+
+Lemma wp_internalSelector__Matches_impl sl cs requirements labels_l ls labels_dq :
+  Forall LabelRequirementV.supported requirements →
+  {{{ sl ↦*□ cs ∗
+      ([∗ list] c;r ∈ cs;requirements, label_requirement_rep c r) ∗
+      labels_set_rep labels_l ls labels_dq
+  }}}
+    (labels.internalSelector__Matchesⁱᵐᵖˡ #sl)
+      #(interface.ok (interface.mk labels.Set' #labels_l))
+  {{{ b, RET #b;
+      sl ↦*□ cs ∗
+      ([∗ list] c;r ∈ cs;requirements, label_requirement_rep c r) ∗
+      labels_set_rep labels_l ls labels_dq ∗
+      ⌜ b = bool_decide (selector_matches requirements ls) ⌝
+  }}}.
+Proof.
+  intros Hsupported.
+  wp_start as "H".
+  iDestruct "H" as "(#Hsl & #Hrequirements & Hlabels)".
+  iDestruct (own_slice_len with "Hsl") as %(Hcs_len1 & Hcs_len2).
+  iDestruct (big_sepL2_length with "Hrequirements") as %Hrequirements_len.
+  rewrite exception_do_unseal /exception_do_def.
+  wp_auto.
+  set I := (∃ (loop_i source_i : w64),
+    "Hloop_i" ∷ i_ptr ↦ loop_i ∗
+    "Hix" ∷ ix_ptr ↦ source_i ∗
+    "Hlabels" ∷ labels_set_rep labels_l ls labels_dq ∗
+    "%Hi_bounds" ∷ ⌜ 0 ≤ sint.Z loop_i ≤ sint.Z (slice.len sl) ⌝ ∗
+    "%Hprefix" ∷ ⌜ selector_matches (take (sint.nat loop_i) requirements) ls ⌝)%I.
+  iAssert I with "[i ix Hlabels]" as "Hloop".
+  { iExists (W64 0), (W64 0). iFrame. iPureIntro.
+    split; [word|constructor]. }
+  wp_for "Hloop". wp_if_destruct.
+  - assert (0 ≤ sint.Z loop_i < sint.Z (slice.len sl)) as Hslice_bounds by word.
+    list_elem cs (sint.Z loop_i) as current_c.
+    assert (∃ current_r, requirements !! sint.nat loop_i = Some current_r)
+      as [current_r Hcurrent_r_lookup].
+    { apply lookup_lt_is_Some_2.
+      rewrite <-Hrequirements_len. rewrite Hcs_len1. word. }
+    iDestruct (big_sepL2_lookup _ _ _ (sint.nat loop_i) current_c current_r
+      with "Hrequirements") as "#Hcurrent";
+      [exact Hcurrent_c_lookup|exact Hcurrent_r_lookup|].
+    iDestruct (own_slice_elem_acc (sint.Z loop_i) with "Hsl")
+      as "[#Hcell _]"; [word|exact Hcurrent_c_lookup|].
+    rewrite -> decide_True by exact Hslice_bounds.
+    wp_apply (wp_load_slice_index (V:=labels.Requirement.t)
+      (t:=labels.Requirement) sl (sint.Z loop_i) cs with "[$Hsl]");
+      [word|iPureIntro; exact Hcurrent_c_lookup|].
+    iIntros "_". wp_auto.
+    rewrite -> decide_True by exact Hslice_bounds.
+    wp_bind ((MethodResolve (go.PointerType labels.Requirement) "Matches"
+      #(slice_index_ref labels.Requirement.t (sint.Z loop_i) sl))
+      #(interface.ok (interface.mk labels.Set' #labels_l)))%E.
+    assert (LabelRequirementV.supported current_r) as Hcurrent_supported.
+    { rewrite Forall_forall in Hsupported. apply Hsupported.
+      rewrite <-list_elem_of_In.
+      eapply list_elem_of_lookup_2. exact Hcurrent_r_lookup. }
+    wp_pures. wp_method_call. wp_call.
+    wp_apply (wp_Requirement__Matches_impl
+      (slice_index_ref labels.Requirement.t (sint.Z loop_i) sl)
+      current_c current_r DfracDiscarded labels_l ls labels_dq Hcurrent_supported with
+      "[$Hcell $Hcurrent $Hlabels]").
+    iIntros (matches) "(_ & _ & Hlabels & %Hmatches)".
+    wp_auto.
+    destruct (decide (LabelRequirementV.matches current_r ls))
+      as [Hcurrent_matches|Hcurrent_not_matches].
+    + rewrite -> bool_decide_true in Hmatches by exact Hcurrent_matches.
+      subst matches. wp_auto.
+      iApply wp_for_post_do. wp_auto.
+      iFrame "HΦ s l Hlabels".
+      iExists (word.add loop_i (W64 1)), loop_i. iFrame.
+      iPureIntro. split; first word.
+      assert (sint.nat (word.add loop_i (W64 1)) = S (sint.nat loop_i)) as -> by word.
+      rewrite (take_S_r _ _ current_r Hcurrent_r_lookup).
+      rewrite /selector_matches Forall_app Forall_singleton.
+      split; first exact Hprefix. exact Hcurrent_matches.
+    + rewrite -> bool_decide_false in Hmatches by exact Hcurrent_not_matches.
+      subst matches. wp_auto.
+      iApply wp_for_post_return.
+      rewrite return_val_unseal /return_val_def. wp_auto.
+      rewrite exception_seq_unseal /exception.exception_seq_def. wp_auto.
+      iApply "HΦ". iFrame "# Hlabels". iPureIntro.
+      assert (¬ selector_matches requirements ls) as Hnot_matches.
+      { intros Hall.
+        rewrite /selector_matches Forall_forall in Hall.
+        specialize (Hall current_r).
+        rewrite <-list_elem_of_In in Hall.
+        assert (current_r ∈ requirements) as Hin_requirement.
+        { eapply list_elem_of_lookup_2. exact Hcurrent_r_lookup. }
+        exact (Hcurrent_not_matches (Hall Hin_requirement)). }
+      rewrite bool_decide_false; done.
+  - assert (sint.nat loop_i = length requirements) as Hi_len.
+    { rewrite <-Hrequirements_len. rewrite Hcs_len1. word. }
+    assert (take (sint.nat loop_i) requirements = requirements) as Htake.
+    { apply take_ge. rewrite Hi_len. done. }
+    rewrite Htake in Hprefix.
+    rewrite return_val_unseal /return_val_def. wp_auto.
+    iApply "HΦ". iFrame "# Hlabels". iPureIntro.
+    rewrite bool_decide_true; done.
+Qed.
+
+Lemma wp_internalSelector__Matches sl cs requirements labels_l ls labels_dq :
+  Forall LabelRequirementV.supported requirements →
+  {{{ sl ↦*□ cs ∗
+      ([∗ list] c;r ∈ cs;requirements, label_requirement_rep c r) ∗
+      labels_set_rep labels_l ls labels_dq
+  }}}
+    sl @! labels.internalSelector @! "Matches"
+      #(interface.ok (interface.mk labels.Set' #labels_l))
+  {{{ b, RET #b;
+      sl ↦*□ cs ∗
+      ([∗ list] c;r ∈ cs;requirements, label_requirement_rep c r) ∗
+      labels_set_rep labels_l ls labels_dq ∗
+      ⌜ b = bool_decide (selector_matches requirements ls) ⌝
+  }}}.
+Proof.
+  intros Hsupported.
+  iIntros (Φ) "H HΦ".
+  wp_method_call. wp_call.
+  wp_apply (wp_internalSelector__Matches_impl sl cs requirements labels_l ls labels_dq
+    Hsupported with "H").
+  iIntros (b) "H". iApply "HΦ". iExact "H".
+Qed.
+
+Lemma wp_Selector__Matches_resolved selector P
+    `{!∀ ls, Decision (P ls)} labels_l ls labels_dq :
+  {{{ is_selector selector P ∗ labels_set_rep labels_l ls labels_dq }}}
+    (match selector with
+    | interface.ok i => Val (#(methods i.(interface.ty) "Matches" i.(interface.v)))
+    | interface.nil => Panic "nil interface"
+    end) #(interface.ok (interface.mk labels.Set' #labels_l))
+  {{{ b, RET #b;
+      is_selector selector P ∗
+      labels_set_rep labels_l ls labels_dq ∗
+      ⌜ b = bool_decide (P ls) ⌝
+  }}}.
+Proof.
+  wp_start as "H".
+  iDestruct "H" as "[#Hselector Hlabels]".
+  rewrite /is_selector.
+  iDestruct "Hselector" as
+    "[(%sl & %cs & %requirements & %Hselector & #Hsl & #Hrequirements &
+       %Hsupported & %HP)|(%Hselector & %HP)]".
+  - subst selector. simpl.
+    wp_apply (wp_internalSelector__Matches sl cs requirements labels_l ls labels_dq
+      Hsupported with "[$Hsl $Hrequirements $Hlabels]").
+    iIntros (b) "(_ & _ & Hlabels & %Hb)".
+    iApply "HΦ". iSplit.
+    { iLeft. iExists sl, cs, requirements. iFrame "#%". done. }
+    iFrame "# Hlabels". iPureIntro.
+    rewrite Hb. apply bool_decide_ext. symmetry. apply HP.
+  - subst selector. simpl.
+    pose proof (labels.nothingSelector_Matches_unfold
+      (nothingSelector_Assumptions:=
+        labels.nothingSelector_instance (Assumptions:=package_sem))) as Hmethod.
+    pose proof (@method_unfold _ _ _ _ _ _ Hmethod) as Hmethod_unfold.
+    iEval (rewrite Hmethod_unfold). wp_call.
+    rewrite /labels.nothingSelector__Matchesⁱᵐᵖˡ. wp_call. wp_auto.
+    iApply "HΦ". iSplit.
+    { iRight. iFrame "#%". done. }
+    iFrame "# Hlabels". iPureIntro.
+    symmetry. apply bool_decide_eq_false_2. apply HP.
+Qed.
+
+Lemma wp_Selector__Matches selector P
+    `{!∀ ls, Decision (P ls)} labels_l ls labels_dq :
+  {{{ is_selector selector P ∗ labels_set_rep labels_l ls labels_dq }}}
+    (MethodResolve labels.Selector "Matches" #selector)
+      #(interface.ok (interface.mk labels.Set' #labels_l))
+  {{{ b, RET #b;
+      is_selector selector P ∗
+      labels_set_rep labels_l ls labels_dq ∗
+      ⌜ b = bool_decide (P ls) ⌝
+  }}}.
+Proof.
+  wp_start as "H".
+  iDestruct "H" as "[#Hselector Hlabels]".
+  rewrite /is_selector.
+  iDestruct "Hselector" as
+    "[(%sl & %cs & %requirements & %Hselector & #Hsl & #Hrequirements &
+       %Hsupported & %HP)|(%Hselector & %HP)]".
+  - subst selector. wp_pures.
+    wp_apply (wp_internalSelector__Matches sl cs requirements labels_l ls labels_dq
+      Hsupported with "[$Hsl $Hrequirements $Hlabels]").
+    iIntros (b) "(_ & _ & Hlabels & %Hb)".
+    iApply "HΦ". iSplit.
+    { iLeft. iExists sl, cs, requirements. iFrame "#%". done. }
+    iFrame "# Hlabels". iPureIntro.
+    rewrite Hb. apply bool_decide_ext. symmetry. apply HP.
+  - subst selector. wp_pures.
+    pose proof (labels.nothingSelector_Matches_unfold
+      (nothingSelector_Assumptions:=
+        labels.nothingSelector_instance (Assumptions:=package_sem))) as Hmethod.
+    pose proof (@method_unfold _ _ _ _ _ _ Hmethod) as Hmethod_unfold.
+    iEval (rewrite Hmethod_unfold). wp_call.
+    rewrite /labels.nothingSelector__Matchesⁱᵐᵖˡ. wp_call. wp_auto.
+    iApply "HΦ". iSplit.
+    { iRight. iFrame "#%". done. }
+    iFrame "# Hlabels". iPureIntro.
+    symmetry. apply bool_decide_eq_false_2. apply HP.
+Qed.
+
+Lemma wp_Everything :
+  {{{ is_pkg_init labels }}}
+    @! labels.Everything #()
+  {{{ selector, RET #selector; is_selector selector everything_matches }}}.
+Proof.
+  wp_start.
+  iDestruct (is_pkg_init_access with "[$]") as "Hinit".
+  simpl. iNamed "Hinit".
+  wp_auto.
+  iApply "HΦ".
+  iLeft.
+  iExists slice.nil, [], [].
+  iSplit; first done.
+  iSplit; first iApply own_slice_nil.
+  iSplit; first done.
+  iSplit; first (iPureIntro; constructor).
+  iPureIntro. intros ls. split; intros; constructor.
+Qed.
+
+Lemma wp_Nothing :
+  {{{ is_pkg_init labels }}}
+    @! labels.Nothing #()
+  {{{ selector, RET #selector; is_selector selector nothing_matches }}}.
+Proof.
+  wp_start.
+  iDestruct (is_pkg_init_access with "[$]") as "Hinit".
+  simpl. iNamed "Hinit".
+  wp_auto.
+  iApply "HΦ".
+  iRight. iSplit; first done.
+  iPureIntro. intros ls Hfalse. unfold nothing_matches in Hfalse.
+  contradiction.
+Qed.
+
+End proof.
