src/proof/k8s_io/apimachinery/pkg/labels_add.v
@@ -1,0 +1,104 @@
+From New.proof Require Import prelude empty_ffi sort.
+From New.proof.k8s_io.apimachinery.pkg Require Export labels_sort.
+
+Section proof.
+Context `{hG: !heapGS Σ} `{!ffi_semantics _ _}.
+Context {sem : go.Semantics} {package_sem : labels.Assumptions}.
+Collection W := sem + package_sem.
+Local Set Default Proof Using "All".
+
+Lemma selector_matches_permutation requirements requirements' :
+  requirements ≡ₚ requirements' →
+  ∀ ls, selector_matches requirements ls ↔
+    selector_matches requirements' ls.
+Proof.
+  intros Hperm ls. rewrite /selector_matches.
+  split; intros Hall.
+  - eapply Permutation_Forall; [exact Hperm|exact Hall].
+  - eapply Permutation_Forall; [symmetry; exact Hperm|exact Hall].
+Qed.
+
+Lemma is_selector_ext selector P Q :
+  (∀ labels_set, P labels_set ↔ Q labels_set) →
+  is_selector selector P -∗ is_selector selector Q.
+Proof.
+  intros HPQ. iIntros "Hselector".
+  iDestruct "Hselector" as
+    "[(%sl & %cs & %requirements & %Hselector & #Hsl & #Hrequirements &
+       %Hsupported & %HP)|(%Hselector & %HP)]".
+  - iLeft. iExists sl, cs, requirements. iFrame "#%".
+    iPureIntro. intros labels_set. rewrite -HP. symmetry. apply HPQ.
+  - iRight. iFrame "%". iPureIntro. intros labels_set HQ.
+    apply (HP labels_set). apply (proj2 (HPQ labels_set)). exact HQ.
+Qed.
+
+Lemma big_sepL_requirement_entries entries :
+  ([∗ list] entry ∈ entries,
+    label_requirement_rep entry.1 entry.2) ⊣⊢
+  ([∗ list] c;r ∈ (fst <$> entries);(snd <$> entries),
+    label_requirement_rep c r).
+Proof.
+  induction entries as [|[c r] entries IH]; simpl; first done.
+  rewrite IH. done.
+Qed.
+
+(** The only receiver produced by [NewSelector] is the empty internal
+    selector.  This specialization proves the complete implementation of
+    [Add] along that controller-relevant path, including both appends and the
+    call to [sort.Sort]. *)
+Lemma wp_empty_internalSelector__Add reqs_sl entries :
+  Z.of_nat (length entries) ≤ 2 ^ 63 - 1 →
+  Forall LabelRequirementV.supported (snd <$> entries) →
+  {{{ is_pkg_init labels ∗
+      by_key_contents reqs_sl entries
+  }}}
+    slice.nil @! labels.internalSelector @! "Add" #reqs_sl
+  {{{ selector, RET #selector;
+      is_selector selector (selector_matches (snd <$> entries))
+  }}}.
+Proof.
+  intros Hsize Hsupported.
+  wp_start as "[Hreqs #Hentries]".
+  iAssert (is_pkg_init sort) as "#Hsort_init".
+  { iPkgInit. }
+  iDestruct (own_slice_len with "Hreqs") as %[Hreqs_len Hreqs_nonnegative].
+  rewrite length_fmap in Hreqs_len.
+  wp_auto.
+  wp_apply (wp_slice_make3 (V:=labels.Requirement.t)
+    (t:=labels.Requirement)); first word.
+  iIntros (ret_sl) "(Hret & Hret_cap & %Hret_cap)".
+  wp_auto.
+  iAssert (slice.nil ↦* ([] : list labels.Requirement.t))%I
+    as "Hsource_nil".
+  { iApply own_slice_nil. }
+  wp_apply (wp_slice_append with "[$Hret $Hret_cap $Hsource_nil]").
+  iIntros (ret_sl') "(Hret & Hret_cap & _)". wp_auto.
+  wp_apply (wp_slice_append with "[$Hret $Hret_cap $Hreqs]").
+  iIntros (ret_sl'') "(Hret & Hret_cap & Hreqs)". wp_auto.
+  iEval (simpl) in "Hret".
+  iAssert (by_key_contents ret_sl'' entries)
+    with "[$Hret $Hentries]" as "Hsort_contents".
+  wp_bind ((let: "$a0" := Convert labels.ByKey sort.Interface #ret_sl'' in
+    (FuncResolve sort.Sort [] #()) "$a0")%E).
+  iApply (wp_Sort labels.ByKey by_key_contents ret_sl'' entries
+    with "[$Hsort_init $Hsort_contents]").
+  iNext.
+  iIntros (sorted_entries) "[Hsort_contents %Hperm]".
+  iDestruct "Hsort_contents" as "[Hret #Hsorted_entries]".
+  iEval (rewrite big_sepL_requirement_entries) in "Hsorted_entries".
+  iMod (own_slice_persist with "Hret") as "#Hret".
+  wp_auto.
+  iApply "HΦ". iLeft.
+  iExists ret_sl'', (fst <$> sorted_entries), (snd <$> sorted_entries).
+  iSplit; first done.
+  iFrame "#".
+  iSplit.
+  { iPureIntro. eapply Permutation_Forall.
+    - apply Permutation_map. exact Hperm.
+    - exact Hsupported. }
+  iPureIntro. intros ls.
+  apply selector_matches_permutation.
+  apply Permutation_map. exact Hperm.
+Qed.
+
+End proof.
