src/proof/k8s_io/apimachinery/pkg/labels_constructor.v
@@ -1,0 +1,235 @@
+From New.proof Require Import prelude empty_ffi sort.
+From New.proof.k8s_io.apimachinery.pkg Require Export labels.
+From New.proof.k8s_io.apimachinery.pkg.util Require Import validation.
+From New.proof.k8s_io.apimachinery.pkg.util.validation Require Import field.
+From New.proof.kubernetes_types Require Import common.
+
+Section proof.
+Context `{hG: !heapGS Σ} `{!ffi_semantics _ _}.
+Context {sem : go.Semantics} {package_sem : labels.Assumptions}.
+Collection W := sem + package_sem.
+Local Set Default Proof Using "All".
+
+Definition valid_requirement_inputs (key : go_string)
+    (operator : selection.Operator.t) (values : list go_string) : Prop :=
+  valid_label_name key ∧
+  Forall valid_label_value values ∧
+  (((operator = "in"%go ∨ operator = "notin"%go) ∧ values ≠ []) ∨
+    (operator = "="%go ∧ length values = 1%nat) ∨
+    ((operator = "exists"%go ∨ operator = "!"%go) ∧
+      values = [])).
+
+Lemma wp_validateLabelKey_valid key (path : loc) :
+  valid_label_name key →
+  {{{ is_pkg_init labels }}}
+    @! labels.validateLabelKey #key #path
+  {{{ RET #null; True }}}.
+Proof.
+  intros Hvalid.
+  wp_start as "#Hinit".
+  iAssert (is_pkg_init validation) as "#Hvalidation_init".
+  { iPkgInit. }
+  wp_auto.
+  wp_apply (wp_IsQualifiedName with "[$Hvalidation_init]").
+  iIntros (sl errs) "[Herrs %Herrs]".
+  apply Herrs in Hvalid. subst errs.
+  iDestruct (own_slice_len with "Herrs") as %[Hlen Hlen_nonnegative].
+  wp_auto.
+  wp_if_destruct.
+  - iApply "HΦ". done.
+  - exfalso. apply n.
+    assert (sint.nat (slice.len sl) = 0%nat) as Hzero.
+    { symmetry. exact Hlen. }
+    word.
+Qed.
+
+Lemma wp_validateLabelValue_valid (key value : go_string) (path : loc) :
+  valid_label_value value →
+  {{{ is_pkg_init labels }}}
+    @! labels.validateLabelValue #key #value #path
+  {{{ RET #null; True }}}.
+Proof.
+  intros Hvalid.
+  wp_start as "#Hinit".
+  iAssert (is_pkg_init validation) as "#Hvalidation_init".
+  { iPkgInit. }
+  wp_auto.
+  wp_apply (wp_IsValidLabelValue with "[$Hvalidation_init]").
+  iIntros (sl errs) "[Herrs %Herrs]".
+  apply Herrs in Hvalid. subst errs.
+  iDestruct (own_slice_len with "Herrs") as %[Hlen Hlen_nonnegative].
+  wp_auto.
+  wp_if_destruct.
+  - iApply "HΦ". done.
+  - exfalso. apply n.
+    assert (sint.nat (slice.len sl) = 0%nat) as Hzero.
+    { symmetry. exact Hlen. }
+    word.
+Qed.
+
+Lemma wp_NewSelector :
+  {{{ True }}}
+    @! labels.NewSelector #()
+  {{{ selector, RET #selector;
+      ⌜ selector = interface.ok
+          (interface.mk labels.internalSelector #slice.nil) ⌝ ∗
+      is_selector selector everything_matches
+  }}}.
+Proof.
+  wp_start as "_".
+  iApply "HΦ". iSplit; first done.
+  iLeft.
+  iExists slice.nil, [], [].
+  iSplit; first done.
+  iSplit; first iApply own_slice_nil.
+  iSplit; first done.
+  iSplit; first (iPureIntro; constructor).
+  iPureIntro. intros ls. split; intros; constructor.
+Qed.
+
+Lemma wp_NewRequirement key operator values_sl values :
+  valid_requirement_inputs key operator values →
+  {{{ is_pkg_init labels ∗ values_sl ↦* values }}}
+    @! labels.NewRequirement #key #operator #values_sl #slice.nil
+  {{{ requirement_l c, RET (#requirement_l, #interface.nil);
+      requirement_l ↦ c ∗
+      label_requirement_rep c (LabelRequirementV.mk key operator values)
+  }}}.
+Proof.
+  intros (Hkey & Hvalues_valid & Harity).
+  wp_start as "Hvalues".
+  iAssert (is_pkg_init labels) as "#Hinit".
+  { iPkgInit. }
+  iAssert (is_pkg_init field) as "#Hfield_init".
+  { iPkgInit. }
+  iDestruct (own_slice_len with "Hvalues") as %[Hvalues_len Hvalues_nonnegative].
+  iMod (own_slice_persist with "Hvalues") as "#Hvalues".
+  wp_auto.
+  wp_apply (wp_ToPath_nil with "[$Hfield_init]").
+  wp_pures.
+  wp_apply (wp_Path__Child null "key"%go with "[$Hfield_init]").
+  iIntros (key_path) "_".
+  wp_pures.
+  wp_apply (wp_validateLabelKey_valid with "[$Hinit]"); first done.
+  wp_pures.
+  wp_apply (wp_Path__Child null "values"%go with "[$Hfield_init]").
+  iIntros (values_path) "_".
+  destruct Harity as
+    [[[Hoperator | Hoperator] Hcardinality] |
+      [[Hoperator Hcardinality] |
+        [[Hoperator | Hoperator] Hcardinality]]].
+  all: rewrite Hoperator.
+  all: lazymatch type of Hcardinality with
+  | ?xs ≠ [] =>
+      assert (slice.len values_sl ≠ W64 0) as Harity_len;
+      [intros Hzero; apply Hcardinality; apply nil_length_inv;
+       rewrite Hvalues_len; word|]
+  | length ?xs = 1%nat =>
+      assert (sint.nat (slice.len values_sl) = 1%nat) as Hnat_len;
+      [rewrite -Hvalues_len; exact Hcardinality|];
+      assert (slice.len values_sl = W64 1) as Harity_len by word
+  | ?xs = [] =>
+      assert (sint.nat (slice.len values_sl) = 0%nat) as Hnat_len;
+      [rewrite -Hvalues_len Hcardinality; done|];
+      assert (slice.len values_sl = W64 0) as Harity_len by word
+  end.
+  all: wp_auto.
+  all: lazymatch type of Harity_len with
+  | ?actual ≠ W64 0 =>
+      rewrite bool_decide_false; try exact Harity_len
+  | ?actual = ?expected =>
+      rewrite Harity_len bool_decide_true; try done
+  end.
+  all: wp_pures.
+  all: wp_auto.
+  all: wp_alloc loop_i_ptr as "Hloop_i"; wp_auto.
+  all: set I := (∃ (loop_i source_i : w64),
+    "Hloop_i" ∷ loop_i_ptr ↦ loop_i ∗
+    "Hi" ∷ i_ptr ↦ source_i ∗
+    "Hvalues" ∷ values_sl ↦*□ values ∗
+    "Hvals" ∷ vals_ptr ↦ values_sl ∗
+    "Hop" ∷ op_ptr ↦ operator ∗
+    "Hkey_ptr" ∷ key_ptr ↦ key ∗
+    "HallErrs" ∷ allErrs_ptr ↦ (zero_val field.ErrorList.t) ∗
+    "HvaluePath" ∷ valuePath_ptr ↦ values_path ∗
+    "%Hloop_bounds" ∷
+      ⌜ 0 ≤ sint.Z loop_i ≤ length values ⌝)%I.
+  Ltac initialize_requirement_loop invariant hop :=
+    iAssert invariant with
+      "[Hloop_i i Hvalues vals op key allErrs valuePath]" as "Hloop";
+    [iExists (W64 0), (W64 0); rewrite hop; iFrame; iFrame "#";
+     iPureIntro; word|].
+  all: initialize_requirement_loop I Hoperator.
+  all: subst I.
+  all: wp_for "Hloop"; wp_if_destruct.
+  all: iDestruct "Hloop" as
+    "(Hi & #Hvalues_loop & Hvals & Hop & Hkey_ptr & HallErrs &
+      HvaluePath & %Hloop_bounds)".
+  all: iNamed "Hi".
+  all: iNamed "Hvals".
+  all: iNamed "Hop".
+  all: iNamed "Hkey_ptr".
+  all: iNamed "HallErrs".
+  all: iNamed "HvaluePath".
+  all: lazymatch goal with
+  | Hbounds : 0 ≤ sint.Z ?idx ≤ _,
+    Hzero : slice.len ?sl = W64 0,
+    Hlt : sint.Z ?idx < sint.Z (slice.len ?sl) |- _ =>
+      destruct Hbounds as [Hloop_nonnegative _];
+      rewrite Hzero in Hlt; exfalso; word
+  | _ => idtac
+  end.
+  all: lazymatch goal with
+  | Hlt : sint.Z ?idx < _ |- _ =>
+      rename Hlt into Hloop_lt;
+      destruct Hloop_bounds as [Hloop_nonnegative Hloop_upper];
+      assert (0 ≤ sint.Z idx < length values) as Hvalue_bounds by word;
+      assert (0 ≤ sint.Z idx < sint.Z (slice.len values_sl))
+        as Hslice_bounds by word;
+      list_elem values (sint.Z idx) as current_value;
+      rewrite decide_True; try exact Hslice_bounds;
+      wp_apply (wp_load_slice_index with "[$Hvalues]");
+        [word|iPureIntro; exact Hcurrent_value_lookup|];
+      iIntros "#Hvalues_read1";
+      wp_auto;
+      rewrite decide_True; try exact Hslice_bounds;
+      wp_apply (wp_load_slice_index with "[$Hvalues]");
+        [word|iPureIntro; exact Hcurrent_value_lookup|];
+      iIntros "#Hvalues_read2";
+      wp_auto;
+      wp_pures;
+      wp_apply (wp_Path__Index values_path idx with "[$Hfield_init]");
+      iIntros (indexed_path) "_";
+      wp_pures;
+      rewrite Forall_forall in Hvalues_valid;
+      assert (valid_label_value current_value) as Hcurrent_valid;
+      [apply Hvalues_valid; rewrite <-list_elem_of_In;
+       eapply list_elem_of_lookup_2; exact Hcurrent_value_lookup|];
+      wp_apply (wp_validateLabelValue_valid key current_value indexed_path
+        with "[$Hinit]"); first exact Hcurrent_valid;
+      wp_pures;
+      iApply wp_for_post_do;
+      wp_auto;
+      iFrame "HΦ";
+      iExists (word.add idx (W64 1)), idx;
+      iFrame;
+      iFrame "#";
+      iPureIntro;
+      word
+  | _ => idtac
+  end.
+  all: wp_auto.
+  all: wp_alloc requirement_l as "Hrequirement".
+  all: wp_pures.
+  all: wp_apply (wp_ErrorList__ToAggregate_nil
+    with "[$Hfield_init $HallErrs]").
+  all: iIntros "HallErrs".
+  all: wp_pures.
+  all: iApply "HΦ".
+  all: iFrame "Hrequirement".
+  all: rewrite /label_requirement_rep /=.
+  all: iFrame "#".
+  all: done.
+Qed.
+
+End proof.
