src/proof/k8s_io/apimachinery/pkg/labels_sort.v
@@ -1,0 +1,155 @@
+From New.proof Require Import prelude empty_ffi sort util.
+From New.proof.k8s_io.apimachinery.pkg Require Export labels_constructor.
+
+Section proof.
+Context `{hG: !heapGS Σ} `{!ffi_semantics _ _}.
+Context {sem : go.Semantics} {package_sem : labels.Assumptions}.
+Collection W := sem + package_sem.
+Local Set Default Proof Using "All".
+
+Definition requirement_entry :=
+  (labels.Requirement.t * LabelRequirementV.t)%type.
+
+Definition by_key_contents (sl : slice.t)
+    (entries : list requirement_entry) : iProp Σ :=
+  sl ↦* (fst <$> entries) ∗
+  ([∗ list] entry ∈ entries,
+    label_requirement_rep entry.1 entry.2).
+
+Lemma wp_ByKey__Len sl entries :
+  {{{ by_key_contents sl entries }}}
+    sl @! labels.ByKey @! "Len" #()
+  {{{ (n : w64), RET #n;
+      by_key_contents sl entries ∗
+      ⌜ sint.nat n = length entries ∧ 0 ≤ sint.Z n ⌝
+  }}}.
+Proof.
+  wp_start as "[Hsl #Hentries]".
+  wp_pures. wp_auto.
+  iDestruct (own_slice_len with "Hsl") as %[Hlen Hnonnegative].
+  iApply "HΦ". iFrame "# Hsl". iPureIntro.
+  rewrite length_fmap in Hlen. split; [symmetry|]; done.
+Qed.
+
+Lemma wp_ByKey__Less sl entries (i j : w64) :
+  0 ≤ sint.Z i < length entries → 0 ≤ sint.Z j < length entries →
+  {{{ by_key_contents sl entries }}}
+    sl @! labels.ByKey @! "Less" #i #j
+  {{{ (b : bool), RET #b; by_key_contents sl entries }}}.
+Proof.
+  intros Hi Hj.
+  destruct Hi as [Hi_nonnegative Hi_upper].
+  destruct Hj as [Hj_nonnegative Hj_upper].
+  wp_start as "[Hsl #Hentries]".
+  wp_pures.
+  iDestruct (own_slice_len with "Hsl") as %[Hlen Hnonnegative].
+  rewrite length_fmap in Hlen.
+  assert (sint.Z (slice.len sl) = Z.of_nat (length entries)) as Hlen_Z.
+  { replace (sint.Z (slice.len sl)) with
+      (Z.of_nat (sint.nat (slice.len sl))) by word.
+    rewrite <-Hlen. done. }
+  wp_auto.
+  assert (∃ ci, (fst <$> entries) !! sint.nat i = Some ci)
+    as [ci Hci_lookup].
+  { apply lookup_lt_is_Some_2. rewrite length_fmap.
+    apply Nat2Z.inj_lt.
+    replace (Z.of_nat (sint.nat i)) with (sint.Z i) by word. exact Hi_upper. }
+  assert (∃ cj, (fst <$> entries) !! sint.nat j = Some cj)
+    as [cj Hcj_lookup].
+  { apply lookup_lt_is_Some_2. rewrite length_fmap.
+    apply Nat2Z.inj_lt.
+    replace (Z.of_nat (sint.nat j)) with (sint.Z j) by word. exact Hj_upper. }
+  rewrite -> decide_True by
+    (split; [exact Hi_nonnegative|rewrite Hlen_Z; exact Hi_upper]).
+  iDestruct (own_slice_elem_acc (sint.Z i) with "Hsl") as
+    "[Hci Hrestore]";
+    [exact Hi_nonnegative|exact Hci_lookup|].
+  wp_auto.
+  iDestruct ("Hrestore" with "Hci") as "Hsl".
+  iEval (rewrite (list_insert_id _ _ _ Hci_lookup)) in "Hsl".
+  rewrite -> decide_True by
+    (split; [exact Hj_nonnegative|rewrite Hlen_Z; exact Hj_upper]).
+  iDestruct (own_slice_elem_acc (sint.Z j) with "Hsl") as
+    "[Hcj Hrestore]";
+    [exact Hj_nonnegative|exact Hcj_lookup|].
+  wp_auto.
+  iDestruct ("Hrestore" with "Hcj") as "Hsl".
+  iEval (rewrite (list_insert_id _ _ _ Hcj_lookup)) in "Hsl".
+  iApply "HΦ". iFrame "# Hsl".
+Qed.
+
+Lemma wp_ByKey__Swap sl entries (i j : w64) :
+  0 ≤ sint.Z i < length entries → 0 ≤ sint.Z j < length entries →
+  {{{ by_key_contents sl entries }}}
+    sl @! labels.ByKey @! "Swap" #i #j
+  {{{ RET #();
+      by_key_contents sl (list_swap entries (sint.nat i) (sint.nat j))
+  }}}.
+Proof.
+  intros Hi Hj.
+  destruct Hi as [Hi_nonnegative Hi_upper].
+  destruct Hj as [Hj_nonnegative Hj_upper].
+  wp_start as "[Hsl #Hentries]".
+  wp_pures.
+  iDestruct (own_slice_len with "Hsl") as %[Hlen Hnonnegative].
+  rewrite length_fmap in Hlen.
+  assert (sint.Z (slice.len sl) = Z.of_nat (length entries)) as Hlen_Z.
+  { replace (sint.Z (slice.len sl)) with
+      (Z.of_nat (sint.nat (slice.len sl))) by word.
+    rewrite <-Hlen. done. }
+  wp_auto.
+  assert (∃ ci, (fst <$> entries) !! sint.nat i = Some ci)
+    as [ci Hci_lookup].
+  { apply lookup_lt_is_Some_2. rewrite length_fmap.
+    apply Nat2Z.inj_lt.
+    replace (Z.of_nat (sint.nat i)) with (sint.Z i) by word. exact Hi_upper. }
+  assert (∃ cj, (fst <$> entries) !! sint.nat j = Some cj)
+    as [cj Hcj_lookup].
+  { apply lookup_lt_is_Some_2. rewrite length_fmap.
+    apply Nat2Z.inj_lt.
+    replace (Z.of_nat (sint.nat j)) with (sint.Z j) by word. exact Hj_upper. }
+  rewrite -> decide_True by
+    (split; [exact Hj_nonnegative|rewrite Hlen_Z; exact Hj_upper]).
+  wp_apply (wp_load_slice_index with "[$Hsl]");
+    [exact Hj_nonnegative|iPureIntro; exact Hcj_lookup|].
+  iIntros "Hsl". wp_auto.
+  rewrite -> decide_True by
+    (split; [exact Hi_nonnegative|rewrite Hlen_Z; exact Hi_upper]).
+  wp_apply (wp_load_slice_index with "[$Hsl]");
+    [exact Hi_nonnegative|iPureIntro; exact Hci_lookup|].
+  iIntros "Hsl". wp_auto.
+  rewrite -> decide_True by
+    (split; [exact Hi_nonnegative|rewrite Hlen_Z; exact Hi_upper]).
+  wp_auto.
+  wp_apply (wp_store_slice_index with "[$Hsl]").
+  { iPureIntro. rewrite length_fmap.
+    split; [exact Hi_nonnegative|exact Hi_upper]. }
+  iIntros "Hsl". wp_auto.
+  rewrite -> decide_True by
+    (split; [exact Hj_nonnegative|rewrite Hlen_Z; exact Hj_upper]).
+  wp_auto.
+  wp_apply (wp_store_slice_index with "[$Hsl]").
+  { iPureIntro. rewrite length_insert length_fmap.
+    split; [exact Hj_nonnegative|exact Hj_upper]. }
+  iIntros "Hsl". wp_auto.
+  iApply "HΦ". rewrite /by_key_contents list_swap_fmap.
+  iSplit.
+  { rewrite /list_swap Hci_lookup Hcj_lookup. iFrame "Hsl". }
+  iEval (rewrite (big_sepL_permutation
+    (fun entry => label_requirement_rep entry.1 entry.2)
+    entries (list_swap entries (sint.nat i) (sint.nat j))
+    (list_swap_permutation entries (sint.nat i) (sint.nat j))))
+    in "Hentries".
+  iFrame "#".
+Qed.
+
+#[global] Instance by_key_sort_interface :
+  SortInterfaceSpec labels.ByKey by_key_contents.
+Proof.
+  constructor.
+  - apply wp_ByKey__Len.
+  - apply wp_ByKey__Less.
+  - apply wp_ByKey__Swap.
+Qed.
+
+End proof.
