src/proof/k8s_io/apimachinery/pkg/util/errors_init.v
@@ -1,0 +1,12 @@
+Require Export New.generatedproof.k8s_io.apimachinery.pkg.util.errors.
+From New.proof Require Import proof_prelude.
+
+Section proof.
+Context `{hG: heapGS Σ} `{!ffi_semantics _ _}.
+Context {sem : go.Semantics} {package_sem : errors.Assumptions}.
+Collection W := sem + package_sem.
+
+#[global] Instance : IsPkgInit (iProp Σ) errors := define_is_pkg_init True%I.
+#[global] Instance : GetIsPkgInitWf (iProp Σ) errors := build_get_is_pkg_init_wf.
+
+End proof.
