src/proof/map/len.v
@@ -1,0 +1,75 @@
+From New.proof Require Import prelude empty_ffi.
+From New.golang.theory Require Export map.
+From iris.algebra Require Import gmap.
+
+Section proof.
+Context `{hG: !heapGS Σ} `{!ffi_semantics _ _}.
+Context {sem : go.Semantics}.
+Local Set Default Proof Using "All".
+
+Context `[!ZeroVal K] `[!EqDecision K] `[!Countable K] `[!ZeroVal V]
+  `[!go.IntoValInj K].
+
+Lemma wp_map_len_resolved key_type elem_type mref (m : gmap K V) dq
+    `{!TypedPointsto K} `{!IntoValTyped K key_type} :
+  {{{ mref ↦${dq} m }}}
+    #(functions go.len [go.MapType key_type elem_type]) #mref
+  {{{ RET #(W64 (size m)); mref ↦${dq} m }}}.
+Proof.
+  wp_start as "Hm".
+  rewrite own_map_unseal. iNamed "Hm".
+  unshelve epose proof (go.is_map_domain_exists mv mp His_map) as
+    [ks Hks_domain].
+  eapply go.is_map_domain_pure in Hks_domain as Hks; last done.
+  destruct Hks as [Hks_nodup Hks].
+  assert (Forall (λ kv, ∃ (k : K), kv = #k) ks) as Heq.
+  { rewrite Forall_forall. intros kv.
+    intros Hkv. specialize (Hks kv). specialize (Hdom kv).
+    rewrite -Hks in Hkv. apply Hdom in Hkv. done. }
+  apply Forall_exists_Forall2_l in Heq as [keys Heq].
+  apply Forall2_fmap_2 in Heq. rewrite -list_eq_Forall2 in Heq.
+  rewrite list_fmap_id in Heq. subst ks.
+  assert (Hkeys_dom : list_to_set keys = dom m).
+  { rewrite sets.set_eq. intros k.
+    rewrite elem_of_list_to_set.
+    specialize (Hks #k). specialize (Hagree k).
+    rewrite list_elem_of_fmap_inj in Hks.
+    rewrite -Hks Hagree elem_of_dom.
+    destruct (m !! k); split; eauto; intros ?; done. }
+  assert (Hkeys_len : length keys = size m).
+  { apply NoDup_fmap in Hks_nodup; last tc_solve.
+    rewrite <- (size_list_to_set (C:=gset K)); last done.
+    rewrite Hkeys_dom size_dom. done. }
+  wp_apply (_internal_wp_untyped_read with "[Hown]") as "Hown".
+  { iExact "Hown". }
+  pose proof (go.internal_map_length_step_pure mv ((λ k : K, #k) <$> keys)
+    Hks_domain) as Hlenstep.
+  wp_auto.
+  iEval (rewrite -Hkeys_len) in "HΦ".
+  rewrite map_length.
+  iApply "HΦ".
+  iExists mv, mp. iFrame "Hown". iFrame "%".
+Qed.
+
+Lemma wp_map_len key_type elem_type mref (m : gmap K V) dq
+    `{!TypedPointsto K} `{!IntoValTyped K key_type} :
+  {{{ mref ↦${dq} m }}}
+    (FuncResolve go.len [go.MapType key_type elem_type] #()) #mref
+  {{{ RET #(W64 (size m)); mref ↦${dq} m }}}.
+Proof.
+  wp_start as "Hm". wp_pures.
+  wp_apply (wp_map_len_resolved with "Hm").
+  iIntros "Hm". iApply "HΦ". iFrame.
+Qed.
+
+Lemma wp_map_len_nil_resolved key_type elem_type :
+  {{{ True }}}
+    #(functions go.len [go.MapType key_type elem_type]) #map.nil
+  {{{ RET #(W64 0); True }}}.
+Proof.
+  (* TODO: Perennial's [MapSemantics] currently has no premise establishing an
+     [is_map_domain] for [map.nil].  Add the corresponding nil-map reduction
+     upstream, then replace this narrow Go-language compatibility boundary. *)
+Admitted.
+
+End proof.
